memory_ops_solvers_impl_soundness.v
@@ -1,0 +1,2411 @@
+Require Import Arith.
+Require Import Nat. 
+Require Import Bool.
+Require Import bbv.Word. 
+Require Import Coq.NArith.NArith.
+Require Import List.
+Import ListNotations.
+Require Import Coq.Logic.FunctionalExtensionality.
+
+Require Import FORVES2.constants.
+Import Constants.
+
+Require Import FORVES2.program.
+Import Program.
+
+Require Import FORVES2.execution_state.
+Import ExecutionState.
+
+Require Import FORVES2.stack_operation_instructions.
+Import StackOpInstrs.
+
+Require Import FORVES2.misc.
+Import Misc.
+
+Require Import FORVES2.symbolic_state.
+Import SymbolicState.
+
+Require Import FORVES2.symbolic_state_eval.
+Import SymbolicStateEval.
+
+Require Import FORVES2.symbolic_state_eval_facts.
+Import SymbolicStateEvalFacts.
+
+Require Import FORVES2.valid_symbolic_state.
+Import ValidSymbolicState.
+
+Require Import FORVES2.memory_ops_solvers.
+Import MemoryOpsSolvers.
+
+Require Import FORVES2.memory_ops_solvers_impl.
+Import MemoryOpsSolversImpl.
+
+Require Import FORVES2.symbolic_state_cmp.
+Import SymbolicStateCmp.
+
+Require Import FORVES2.symbolic_execution_soundness.
+Import SymbolicExecutionSoundness.
+
+Require Import storage_ops_solvers_impl_soundness.
+Import StorageOpsSolversImplSoundness.
+
+Require Import memory_ops_solvers_impl_soundness_misc.
+Import MemoryOpsSolversImplSoundnessMisc.
+
+Require Import FORVES2.constraints.
+Import Constraints.
+
+Module MemoryOpsSolversImplSoundness.
+
+  Lemma trivial_mload_solver_snd: mload_solver_ext_snd trivial_mload_solver.
+  Proof.
+    unfold mload_solver_ext_snd.
+    unfold mload_solver_snd.
+    intros.
+    split.
+    - unfold mload_solver_valid_res.
+      intros.
+      unfold trivial_mload_solver in H3.
+      rewrite <- H3.
+      simpl.
+      intuition.
+    - unfold mload_solver_correct_res.
+      intros.
+      unfold trivial_mload_solver in H4.
+      rewrite <- H4 in H5.
+      rewrite H5.
+      exists idx1.
+      exists m1.
+      split; try reflexivity.
+      intros.
+      unfold eval_sstack_val.
+      symmetry in H6.
+
+      assert (H_valid_smap_value: valid_smap_value (get_maxidx_smap m) ops (SymMLOAD soffset smem)). simpl. intuition.
+
+      symmetry in H5.
+      pose proof (add_to_smap_key_lt_maxidx m m1 idx1 (SymMLOAD soffset smem) H5).
+      pose proof (valid_sstack_val_freshvar (get_maxidx_smap m1) idx1 H7).
+      symmetry in H5.
+      pose proof (add_to_smap_valid_smap idx1 m m1 (SymMLOAD soffset smem) ops H1 H_valid_smap_value H5).
+      pose proof (eval_sstack_val'_succ (S (get_maxidx_smap m1)) (FreshVar idx1) model mem strg exts (get_maxidx_smap m1) (get_bindings_smap m1) ops H8 H9 (gt_Sn_n (get_maxidx_smap m1))).
+      destruct H10 as [v H10].
+      exists v.
+      split; apply H10.
+  Qed.
+  
+  Lemma trivial_smemory_updater_snd: smemory_updater_ext_snd trivial_smemory_updater.
+  Proof.
+    unfold smemory_updater_ext_snd.
+    intros sstack_val_cmp H_valid_sstack_val_cmp.
+    unfold smemory_updater_snd.
+    split.
+    - unfold smemory_updater_valid_res.
+      intros ctx m smem smem' u ops H_is_sat H_valid_smem H_valid_u H_updater.
+      unfold trivial_smemory_updater in H_updater.
+      rewrite <- H_updater.
+      simpl.
+      split.
+      + apply H_valid_u.
+      + apply H_valid_smem.
+    - unfold smemory_updater_correct_res.
+      intros ctx m smem smem' u ops H_is_sat H_valid_smap H_valid_smem H_valid_u H_updater.
+      unfold trivial_smemory_updater in H_updater.
+      rewrite <- H_updater.
+      intros model mem strg exts H_is_model.
+      pose proof (valid_smemory_when_extended_with_valid_update (get_maxidx_smap m) u smem H_valid_u H_valid_smem) as H_valid_u_smem.
+      unfold valid_smap in H_valid_smap.
+      pose proof (eval_smemory_succ (get_maxidx_smap m) (get_bindings_smap m) model mem strg exts ops (u::smem) H_valid_u_smem H_valid_smap) as H_eval_smemory_u_smem.
+      destruct H_eval_smemory_u_smem as [smem'' H_eval_smemory_u_smem].
+      exists smem''.
+      exists smem''.
+      repeat split; apply H_eval_smemory_u_smem.
+  Qed.
+
+Lemma  H_memory_slots_do_not_overlap:
+    forall ctx soffset soffset' size size' maxidx sbindings ops,
+      valid_bindings maxidx sbindings ops ->
+      valid_sstack_value maxidx soffset  ->
+      valid_sstack_value maxidx soffset' ->
+      memory_slots_do_not_overlap ctx soffset soffset' size size' maxidx sbindings ops = true ->
+      forall model mem strg exts,
+        is_model ctx model = true ->
+        exists v1 v2,
+        eval_sstack_val' (S maxidx) soffset model mem strg exts maxidx sbindings ops = Some v1 /\
+          eval_sstack_val' (S maxidx) soffset' model mem strg exts maxidx sbindings ops = Some v2 /\
+          orb ((wordToN v1)+size <? (wordToN v2))%N ((wordToN v2) + size' <? (wordToN v1))%N = true.
+  Proof.
+    intros ctx soffset soffset' size size' maxidx sbindings ops.
+    intros H_valid_sbindings H_valid_offset H_valid_offset' H_addr_nover.
+    unfold memory_slots_do_not_overlap in H_addr_nover.
+    
+    destruct (follow_in_smap soffset maxidx sbindings) as [soffset_m|] eqn:E_follow_soffset; try discriminate.
+    destruct soffset_m; try discriminate.
+    destruct smv; try discriminate.
+    destruct val; try discriminate.
+
+    destruct (follow_in_smap soffset' maxidx sbindings) as [soffset'_m|] eqn:E_follow_soffset'; try discriminate.
+    destruct soffset'_m; try discriminate.
+    destruct smv; try discriminate.
+    destruct val0; try discriminate.
+
+    intros modfe mem strg exts.
+    intros H_is_model.
+    unfold eval_sstack_val' at 1.
+    rewrite E_follow_soffset.
+    unfold eval_sstack_val' at 1.
+    rewrite E_follow_soffset'.
+    exists val.
+    exists val0.
+    split; try split; try reflexivity.
+    apply H_addr_nover.
+  Qed.
+
+  Lemma  H_mstore8_is_included_in_mstore:
+    forall sstack_val_cmp ctx soffset_mstore8 soffset_mstore maxidx sbindings ops,
+      safe_sstack_val_cmp_ext_1 sstack_val_cmp ->
+      valid_bindings maxidx sbindings ops ->
+      valid_sstack_value maxidx soffset_mstore8  ->
+      valid_sstack_value maxidx soffset_mstore ->
+      mstore8_is_included_in_mstore sstack_val_cmp ctx soffset_mstore8 soffset_mstore maxidx sbindings ops = true ->
+      forall model mem strg exts,
+        is_model ctx model = true ->
+        exists v1 v2,
+        eval_sstack_val' (S maxidx) soffset_mstore8 model mem strg exts maxidx sbindings ops = Some v1 /\
+          eval_sstack_val' (S maxidx) soffset_mstore model mem strg exts maxidx sbindings ops = Some v2 /\
+          andb ((wordToN v2) <=? (wordToN v1) )%N ((wordToN v1) <=? (wordToN v2)+31)%N = true.
+  Proof.
+    intros sstack_val_cmp ctx soffset_mstore8 soffset_mstore maxidx sbindings ops.
+    intros H_sstack_val_cmp_snd H_valid_sbindings H_valid_offset_mstore8 H_valid_offset_mstore H_addr_not_inc.
+    unfold mstore8_is_included_in_mstore in H_addr_not_inc.
+
+    destruct (follow_in_smap soffset_mstore8 maxidx sbindings) as [soffset_mstore8_m|] eqn:E_follow_soffset_mstore8; try discriminate.
+    destruct soffset_mstore8_m; try discriminate.
+    destruct smv; try discriminate.
+    destruct val; try discriminate.
+
+    destruct (follow_in_smap soffset_mstore maxidx sbindings) as [soffset_mstore_m|] eqn:E_follow_soffset_mstore; try discriminate.
+    destruct soffset_mstore_m; try discriminate.
+    destruct smv; try discriminate.
+    destruct val0; try discriminate.
+
+    intros model mem strg exts.
+    intros H_is_model.
+    unfold eval_sstack_val' at 1.
+    rewrite E_follow_soffset_mstore8.
+    unfold eval_sstack_val' at 1.
+    rewrite E_follow_soffset_mstore.
+    exists val.
+    exists val0.
+    split; try split; try reflexivity.
+    apply H_addr_not_inc.
+  Qed.
+
+  Lemma basic_mload_solver_valid:
+    forall sstack_val_cmp,
+      mload_solver_valid_res (basic_mload_solver sstack_val_cmp).
+  Proof.
+    intros sstack_val_cmp.
+    unfold mload_solver_valid_res.
+    intros ctx m smem soffset smv ops H_is_sat H_valid_smem H_valid_offset.
+    revert H_valid_smem.
+    revert smem.
+    induction smem as [|u smem' IHsmem'].
+    + intros H_valid_smem H_basic_solver.
+      simpl in H_basic_solver.
+      rewrite <- H_basic_solver.
+      simpl.
+      split; auto.
+    + intros H_valid_smem H_basic_solver.
+      simpl in H_basic_solver.
+      destruct u as [soffset' svalue|].
+      ++ destruct (sstack_val_cmp (S (get_maxidx_smap m)) ctx soffset soffset' (get_maxidx_smap m) (get_bindings_smap m) (get_maxidx_smap m) (get_bindings_smap m) ops) eqn:E_soffset_soffset'_cmp.
+         +++ rewrite <- H_basic_solver.
+             simpl.
+             apply H_valid_smem.
+         +++ destruct (memory_slots_do_not_overlap ctx soffset soffset' 31 31) eqn:E_do_not_overlap.
+             ++++ apply IHsmem'.
+                  apply H_valid_smem.
+                  apply H_basic_solver.
+             ++++ rewrite <- H_basic_solver.
+                  simpl.
+                  split; auto.
+      ++ destruct (memory_slots_do_not_overlap ctx soffset offset 31 0) eqn:E_do_not_overlap.
+         +++ apply IHsmem'.
+             apply H_valid_smem.
+             apply H_basic_solver.
+         +++ rewrite <- H_basic_solver.
+             simpl.
+             split; auto.
+  Qed.
+
+
+  Lemma S_S_n_gt_n: forall n, S (S n) > n.
+  Proof.
+    auto.
+  Qed.
+  
+
+                                                                                               
+Lemma H_map_o_smem:
+  forall ctx d model mem strg exts maxidx bs ops smem,
+    valid_smemory maxidx smem ->
+    valid_bindings maxidx bs ops ->
+    d > maxidx ->
+    is_model ctx model = true ->
+    exists v,
+      map_option (eval_common.EvalCommon.instantiate_memory_update (fun sv : sstack_val => eval_sstack_val' d sv model mem strg exts maxidx bs ops)) smem = Some v.
+Proof.
+induction smem as [|u sstrg' IHsstrg'].
++ intros. simpl. exists []. reflexivity.
++ intros H_valid_smemory H_valid_bs H_d_gt_maxidx H_is_model.
+  unfold map_option.
+  rewrite <- map_option_ho.
+  unfold eval_common.EvalCommon.instantiate_memory_update at 1.
+  destruct u as [soffset' svalue' | soffset' svalue'].
+
+  ++ unfold valid_smemory in H_valid_smemory. fold valid_smemory in H_valid_smemory.
+     destruct H_valid_smemory as [H_valid_smemory_0 H_valid_smemory_1].
+     unfold valid_smemory_update in H_valid_smemory_0.
+     destruct H_valid_smemory_0 as [H_valid_smemory_0_0 H_valid_smemory_0_1].
+
+     pose proof (eval_sstack_val'_succ d soffset' model mem strg exts maxidx bs ops H_valid_smemory_0_0 H_valid_bs H_d_gt_maxidx) as eval_sstack_val'_succ_0.
+  
+     destruct eval_sstack_val'_succ_0 as [v eval_sstack_val'_succ_0].
+     rewrite eval_sstack_val'_succ_0.
+     pose proof (eval_sstack_val'_succ d svalue' model mem strg exts maxidx bs ops H_valid_smemory_0_1 H_valid_bs H_d_gt_maxidx) as eval_sstack_val'_succ_1.
+     destruct eval_sstack_val'_succ_1 as [v' eval_sstack_val'_succ_1].
+     rewrite eval_sstack_val'_succ_1.
+
+     pose proof (IHsstrg' H_valid_smemory_1 H_valid_bs H_d_gt_maxidx H_is_model) as IHsstrg'_0.
+     destruct IHsstrg'_0 as [v'' IHsstrg'_0].
+     rewrite IHsstrg'_0.
+     exists (U_MSTORE EVMWord v v' :: v'').
+     reflexivity.
+  ++ unfold valid_smemory in H_valid_smemory. fold valid_smemory in H_valid_smemory.
+     destruct H_valid_smemory as [H_valid_smemory_0 H_valid_smemory_1].
+     unfold valid_smemory_update in H_valid_smemory_0.
+     destruct H_valid_smemory_0 as [H_valid_smemory_0_0 H_valid_smemory_0_1].
+
+     pose proof (eval_sstack_val'_succ d soffset' model mem strg exts maxidx bs ops H_valid_smemory_0_0 H_valid_bs H_d_gt_maxidx) as eval_sstack_val'_succ_0.
+  
+     destruct eval_sstack_val'_succ_0 as [v eval_sstack_val'_succ_0].
+     rewrite eval_sstack_val'_succ_0.
+     pose proof (eval_sstack_val'_succ d svalue' model mem strg exts maxidx bs ops H_valid_smemory_0_1 H_valid_bs H_d_gt_maxidx) as eval_sstack_val'_succ_1.
+     destruct eval_sstack_val'_succ_1 as [v' eval_sstack_val'_succ_1].
+     rewrite eval_sstack_val'_succ_1.
+
+     pose proof (IHsstrg' H_valid_smemory_1 H_valid_bs H_d_gt_maxidx H_is_model) as IHsstrg'_0.
+     destruct IHsstrg'_0 as [v'' IHsstrg'_0].
+     rewrite IHsstrg'_0.
+     exists (U_MSTORE8 EVMWord v v' :: v'').
+     reflexivity.
+  Qed.
+
+ 
+Lemma mstore'_aux:
+  forall sz addr (value : word (sz * 8)) mem,
+    (fix mstore' (sz : nat) (mem0 : memory) {struct sz} : word (sz * 8) -> N -> memory :=
+         match sz as sz0 return (word (sz0 * 8) -> N -> memory) with
+         | 0 => fun (_ : word (0 * 8)) (_ : N) => mem0
+         | S sz1' =>
+             fun (value0 : word (S sz1' * 8)) (offset offset'0 : N) =>
+             if (offset'0 =? offset)%N
+             then concrete_interpreter.ConcreteInterpreter.split1_byte value0
+             else mstore' sz1' mem0 (concrete_interpreter.ConcreteInterpreter.split2_byte value0) (offset + 1)%N offset'0
+         end) sz mem value addr = concrete_interpreter.ConcreteInterpreter.mstore' mem value addr.
+Proof.
+  auto.
+Qed.
+
+Lemma mload''_aux:
+  forall n addr addr' x y,
+      (addr' > addr)%N ->
+         (concrete_interpreter.ConcreteInterpreter.mload''
+            (fun offset' : N =>
+               if (offset' =? addr)%N
+               then x
+               else y offset') addr' n) =
+           (concrete_interpreter.ConcreteInterpreter.mload'' y addr' n).
+Proof.
+  induction n as [|n' IHn'].
+  + intros.
+    simpl.
+    reflexivity.
+  + intros addr addr' x y H_addr'_gt_addr'.
+    unfold concrete_interpreter.ConcreteInterpreter.mload'' at 1.
+    fold concrete_interpreter.ConcreteInterpreter.mload''.
+
+    assert (H_addr'_neqb_addr: (addr' =? addr)%N = false).
+      (* proof of assert *)
+      rewrite N.eqb_neq.
+      intuition.
+    
+      assert (H_addr'_1_gt_addr: (addr'+1> addr)%N).
+      apply N.lt_gt.
+      apply N.lt_lt_add_r.
+      apply N.gt_lt in H_addr'_gt_addr'.
+      apply H_addr'_gt_addr'.
+      (****)
+      
+    rewrite H_addr'_neqb_addr.
+    unfold concrete_interpreter.ConcreteInterpreter.mload'' at 2.
+    fold concrete_interpreter.ConcreteInterpreter.mload''.
+
+    pose proof (IHn' addr (addr'+1)%N x y H_addr'_1_gt_addr) as IHn'_0.
+    rewrite IHn'_0.
+    reflexivity.
+Qed.
+
+
+
+Lemma mload''_mstore'_same_address:
+  forall n mem addr value,
+  concrete_interpreter.ConcreteInterpreter.mload'' (concrete_interpreter.ConcreteInterpreter.mstore' mem (value: word (n*8)) addr) addr n = value.
+Proof.
+  induction n as [|n' IHn'].
+  + intros mem addr value.
+    simpl.
+    rewrite word0.
+    reflexivity.
+  + intros mem addr value.
+    unfold concrete_interpreter.ConcreteInterpreter.mstore'.
+    rewrite mstore'_aux.
+    unfold concrete_interpreter.ConcreteInterpreter.mload''.
+    rewrite N.eqb_refl.
+    fold concrete_interpreter.ConcreteInterpreter.mload''.
+
+    destruct n' as [|n''] eqn:E_n'.
+    ++ unfold concrete_interpreter.ConcreteInterpreter.mload''.
+       unfold concrete_interpreter.ConcreteInterpreter.split1_byte.
+       unfold concrete_interpreter.ConcreteInterpreter.split1_byte.
+       unfold mul.
+              
+       pose proof (wordToZ_combine_WO (split1 8 0 value)) as H_wordToZ_combine_WO.
+       apply wordToZ_inj in H_wordToZ_combine_WO.
+       rewrite H_wordToZ_combine_WO at 1.
+       
+       pose proof (split1_0 value) as H_split1_0_0.
+       unfold mul in H_split1_0_0.
+       unfold add in H_split1_0_0.
+       pose proof (H_split1_0_0 (eq_refl 8)) as H_split1_0_1.
+       unfold eq_rect in H_split1_0_1.
+       apply H_split1_0_1.
+       
+    ++ rewrite mload''_aux.
+       +++ pose proof (IHn' mem (addr+1)%N (concrete_interpreter.ConcreteInterpreter.split2_byte value)) as IHn'_0.
+           rewrite IHn'_0.
+           unfold concrete_interpreter.ConcreteInterpreter.split1_byte.
+           unfold concrete_interpreter.ConcreteInterpreter.split2_byte.
+           apply Word.combine_split.
+       +++ apply N.lt_gt.
+           apply Nlt_in.
+           rewrite N2Nat.inj_add.
+           simpl.
+           intuition.
+Qed.
+
+Lemma mload_mstore_same_address:
+  forall mem addr value,
+    (concrete_interpreter.ConcreteInterpreter.mload
+       (concrete_interpreter.ConcreteInterpreter.mstore mem value addr) addr) = value.
+Proof.
+  intros mem addr value.
+  unfold concrete_interpreter.ConcreteInterpreter.mload.
+  unfold concrete_interpreter.ConcreteInterpreter.mload'.
+  unfold concrete_interpreter.ConcreteInterpreter.mstore.
+  apply mload''_mstore'_same_address.
+Qed.
+
+ 
+
+
+Lemma do_not_overlap_mload:
+  forall mem offset offset' value' updates,
+    (wordToN offset + 31 <? wordToN offset')%N || (wordToN offset' + 31 <? wordToN offset)%N = true ->
+    (concrete_interpreter.ConcreteInterpreter.mload'' (eval_common.EvalCommon.update_memory mem (U_MSTORE EVMWord offset' value' :: updates)) (wordToN offset) 32) =
+    (concrete_interpreter.ConcreteInterpreter.mload'' (eval_common.EvalCommon.update_memory mem  updates) (wordToN (offset : EVMWord)) 32).
+Proof.
+  intros mem offset offset' value' updates H_o.
+  unfold concrete_interpreter.ConcreteInterpreter.mload''.
+
+  rewrite assoc_ones_31.
+  rewrite Reduce_ones_31.
+
+  rewrite assoc_ones_30.
+  rewrite Reduce_ones_30.
+
+  rewrite assoc_ones_29.
+  rewrite Reduce_ones_29.
+
+  rewrite assoc_ones_28.
+  rewrite Reduce_ones_28.
+
+  rewrite assoc_ones_27.
+  rewrite Reduce_ones_27.
+
+  rewrite assoc_ones_26.
+  rewrite Reduce_ones_26.
+
+  rewrite assoc_ones_25.
+  rewrite Reduce_ones_25.
+
+  rewrite assoc_ones_24.
+  rewrite Reduce_ones_24.
+
+  rewrite assoc_ones_23.
+  rewrite Reduce_ones_23.
+
+  rewrite assoc_ones_22.
+  rewrite Reduce_ones_22.
+
+  rewrite assoc_ones_21.
+  rewrite Reduce_ones_21.
+
+  rewrite assoc_ones_20.
+  rewrite Reduce_ones_20.
+
+  rewrite assoc_ones_19.
+  rewrite Reduce_ones_19.
+
+  rewrite assoc_ones_18.
+  rewrite Reduce_ones_18.
+
+  rewrite assoc_ones_17.
+  rewrite Reduce_ones_17.
+
+  rewrite assoc_ones_16.
+  rewrite Reduce_ones_16.
+
+  rewrite assoc_ones_15.
+  rewrite Reduce_ones_15.
+
+  rewrite assoc_ones_14.
+  rewrite Reduce_ones_14.
+
+  rewrite assoc_ones_13.
+  rewrite Reduce_ones_13.
+
+  rewrite assoc_ones_12.
+  rewrite Reduce_ones_12.
+
+  rewrite assoc_ones_11.
+  rewrite Reduce_ones_11.
+
+  rewrite assoc_ones_10.
+  rewrite Reduce_ones_10.
+
+    rewrite assoc_ones_9.
+  rewrite Reduce_ones_9.
+
+  rewrite assoc_ones_8.
+  rewrite Reduce_ones_8.
+
+  rewrite assoc_ones_7.
+  rewrite Reduce_ones_7.
+
+  rewrite assoc_ones_6.
+  rewrite Reduce_ones_6.
+
+  rewrite assoc_ones_5.
+  rewrite Reduce_ones_5.
+
+  rewrite assoc_ones_4.
+  rewrite Reduce_ones_4.
+
+  rewrite assoc_ones_3.
+  rewrite Reduce_ones_3.
+
+  rewrite assoc_ones_2.
+  rewrite Reduce_ones_2.
+
+
+  rewrite (do_not_overlap_mload_aux mem value' updates 1 offset offset' H_31_lt_32 H_o).
+  rewrite (do_not_overlap_mload_aux mem value' updates 2 offset offset' H_31_lt_32 H_o).
+  rewrite (do_not_overlap_mload_aux mem value' updates 3 offset offset' H_31_lt_32 H_o).
+  rewrite (do_not_overlap_mload_aux mem value' updates 4 offset offset' H_31_lt_32 H_o).
+  rewrite (do_not_overlap_mload_aux mem value' updates 5 offset offset' H_31_lt_32 H_o).
+  rewrite (do_not_overlap_mload_aux mem value' updates 6 offset offset' H_31_lt_32 H_o).
+  rewrite (do_not_overlap_mload_aux mem value' updates 7 offset offset' H_31_lt_32 H_o).
+  rewrite (do_not_overlap_mload_aux mem value' updates 8 offset offset' H_31_lt_32 H_o).
+  rewrite (do_not_overlap_mload_aux mem value' updates 9 offset offset' H_31_lt_32 H_o).
+  rewrite (do_not_overlap_mload_aux mem value' updates 10 offset offset' H_31_lt_32 H_o).
+  rewrite (do_not_overlap_mload_aux mem value' updates 11 offset offset' H_31_lt_32 H_o).
+  rewrite (do_not_overlap_mload_aux mem value' updates 12 offset offset' H_31_lt_32 H_o).
+  rewrite (do_not_overlap_mload_aux mem value' updates 13 offset offset' H_31_lt_32 H_o).
+  rewrite (do_not_overlap_mload_aux mem value' updates 14 offset offset' H_31_lt_32 H_o).
+  rewrite (do_not_overlap_mload_aux mem value' updates 15 offset offset' H_31_lt_32 H_o).
+  rewrite (do_not_overlap_mload_aux mem value' updates 16 offset offset' H_31_lt_32 H_o).
+  rewrite (do_not_overlap_mload_aux mem value' updates 17 offset offset' H_31_lt_32 H_o).
+  rewrite (do_not_overlap_mload_aux mem value' updates 18 offset offset' H_31_lt_32 H_o).
+  rewrite (do_not_overlap_mload_aux mem value' updates 19 offset offset' H_31_lt_32 H_o).
+  rewrite (do_not_overlap_mload_aux mem value' updates 20 offset offset' H_31_lt_32 H_o).
+  rewrite (do_not_overlap_mload_aux mem value' updates 21 offset offset' H_31_lt_32 H_o).
+  rewrite (do_not_overlap_mload_aux mem value' updates 22 offset offset' H_31_lt_32 H_o).
+  rewrite (do_not_overlap_mload_aux mem value' updates 23 offset offset' H_31_lt_32 H_o).
+  rewrite (do_not_overlap_mload_aux mem value' updates 24 offset offset' H_31_lt_32 H_o).
+  rewrite (do_not_overlap_mload_aux mem value' updates 25 offset offset' H_31_lt_32 H_o).
+  rewrite (do_not_overlap_mload_aux mem value' updates 26 offset offset' H_31_lt_32 H_o).
+  rewrite (do_not_overlap_mload_aux mem value' updates 27 offset offset' H_31_lt_32 H_o).
+  rewrite (do_not_overlap_mload_aux mem value' updates 28 offset offset' H_31_lt_32 H_o).
+  rewrite (do_not_overlap_mload_aux mem value' updates 29 offset offset' H_31_lt_32 H_o).
+  rewrite (do_not_overlap_mload_aux mem value' updates 30 offset offset' H_31_lt_32 H_o).
+  rewrite (do_not_overlap_mload_aux mem value' updates 31 offset offset' H_31_lt_32 H_o).
+
+  assert ( H_O_0: (wordToN offset + 0 = wordToN offset)%N). apply N.add_0_r.
+  rewrite <- H_O_0.
+  rewrite (do_not_overlap_mload_aux mem value' updates 0 offset offset' H_31_lt_32 H_o).
+  reflexivity.
+Qed.
+
+Lemma do_not_overlap_mload_0:
+  forall mem offset offset' value' updates,
+    (wordToN offset + 31 <? wordToN offset')%N || (wordToN offset' + 0 <? wordToN offset)%N = true ->
+    (concrete_interpreter.ConcreteInterpreter.mload'' (eval_common.EvalCommon.update_memory mem (U_MSTORE8 EVMWord offset' value' :: updates)) (wordToN offset) 32) =
+    (concrete_interpreter.ConcreteInterpreter.mload'' (eval_common.EvalCommon.update_memory mem  updates) (wordToN (offset : EVMWord)) 32).
+Proof.
+Proof.
+  intros mem offset offset' value' updates H_o.
+  unfold concrete_interpreter.ConcreteInterpreter.mload''.
+
+  rewrite assoc_ones_31.
+  rewrite Reduce_ones_31.
+
+  rewrite assoc_ones_30.
+  rewrite Reduce_ones_30.
+
+  rewrite assoc_ones_29.
+  rewrite Reduce_ones_29.
+
+  rewrite assoc_ones_28.
+  rewrite Reduce_ones_28.
+
+  rewrite assoc_ones_27.
+  rewrite Reduce_ones_27.
+
+  rewrite assoc_ones_26.
+  rewrite Reduce_ones_26.
+
+  rewrite assoc_ones_25.
+  rewrite Reduce_ones_25.
+
+  rewrite assoc_ones_24.
+  rewrite Reduce_ones_24.
+
+  rewrite assoc_ones_23.
+  rewrite Reduce_ones_23.
+
+  rewrite assoc_ones_22.
+  rewrite Reduce_ones_22.
+
+  rewrite assoc_ones_21.
+  rewrite Reduce_ones_21.
+
+  rewrite assoc_ones_20.
+  rewrite Reduce_ones_20.
+
+  rewrite assoc_ones_19.
+  rewrite Reduce_ones_19.
+
+  rewrite assoc_ones_18.
+  rewrite Reduce_ones_18.
+
+  rewrite assoc_ones_17.
+  rewrite Reduce_ones_17.
+
+  rewrite assoc_ones_16.
+  rewrite Reduce_ones_16.
+
+  rewrite assoc_ones_15.
+  rewrite Reduce_ones_15.
+
+  rewrite assoc_ones_14.
+  rewrite Reduce_ones_14.
+
+  rewrite assoc_ones_13.
+  rewrite Reduce_ones_13.
+
+  rewrite assoc_ones_12.
+  rewrite Reduce_ones_12.
+
+  rewrite assoc_ones_11.
+  rewrite Reduce_ones_11.
+
+  rewrite assoc_ones_10.
+  rewrite Reduce_ones_10.
+
+    rewrite assoc_ones_9.
+  rewrite Reduce_ones_9.
+
+  rewrite assoc_ones_8.
+  rewrite Reduce_ones_8.
+
+  rewrite assoc_ones_7.
+  rewrite Reduce_ones_7.
+
+  rewrite assoc_ones_6.
+  rewrite Reduce_ones_6.
+
+  rewrite assoc_ones_5.
+  rewrite Reduce_ones_5.
+
+  rewrite assoc_ones_4.
+  rewrite Reduce_ones_4.
+
+  rewrite assoc_ones_3.
+  rewrite Reduce_ones_3.
+
+  rewrite assoc_ones_2.
+  rewrite Reduce_ones_2.
+
+
+  rewrite (do_not_overlap_mload_aux' mem value' updates 1 offset offset' H_31_lt_32 H_o).
+  rewrite (do_not_overlap_mload_aux' mem value' updates 2 offset offset' H_31_lt_32 H_o).
+  rewrite (do_not_overlap_mload_aux' mem value' updates 3 offset offset' H_31_lt_32 H_o).
+  rewrite (do_not_overlap_mload_aux' mem value' updates 4 offset offset' H_31_lt_32 H_o).
+  rewrite (do_not_overlap_mload_aux' mem value' updates 5 offset offset' H_31_lt_32 H_o).
+  rewrite (do_not_overlap_mload_aux' mem value' updates 6 offset offset' H_31_lt_32 H_o).
+  rewrite (do_not_overlap_mload_aux' mem value' updates 7 offset offset' H_31_lt_32 H_o).
+  rewrite (do_not_overlap_mload_aux' mem value' updates 8 offset offset' H_31_lt_32 H_o).
+  rewrite (do_not_overlap_mload_aux' mem value' updates 9 offset offset' H_31_lt_32 H_o).
+  rewrite (do_not_overlap_mload_aux' mem value' updates 10 offset offset' H_31_lt_32 H_o).
+  rewrite (do_not_overlap_mload_aux' mem value' updates 11 offset offset' H_31_lt_32 H_o).
+  rewrite (do_not_overlap_mload_aux' mem value' updates 12 offset offset' H_31_lt_32 H_o).
+  rewrite (do_not_overlap_mload_aux' mem value' updates 13 offset offset' H_31_lt_32 H_o).
+  rewrite (do_not_overlap_mload_aux' mem value' updates 14 offset offset' H_31_lt_32 H_o).
+  rewrite (do_not_overlap_mload_aux' mem value' updates 15 offset offset' H_31_lt_32 H_o).
+  rewrite (do_not_overlap_mload_aux' mem value' updates 16 offset offset' H_31_lt_32 H_o).
+  rewrite (do_not_overlap_mload_aux' mem value' updates 17 offset offset' H_31_lt_32 H_o).
+  rewrite (do_not_overlap_mload_aux' mem value' updates 18 offset offset' H_31_lt_32 H_o).
+  rewrite (do_not_overlap_mload_aux' mem value' updates 19 offset offset' H_31_lt_32 H_o).
+  rewrite (do_not_overlap_mload_aux' mem value' updates 20 offset offset' H_31_lt_32 H_o).
+  rewrite (do_not_overlap_mload_aux' mem value' updates 21 offset offset' H_31_lt_32 H_o).
+  rewrite (do_not_overlap_mload_aux' mem value' updates 22 offset offset' H_31_lt_32 H_o).
+  rewrite (do_not_overlap_mload_aux' mem value' updates 23 offset offset' H_31_lt_32 H_o).
+  rewrite (do_not_overlap_mload_aux' mem value' updates 24 offset offset' H_31_lt_32 H_o).
+  rewrite (do_not_overlap_mload_aux' mem value' updates 25 offset offset' H_31_lt_32 H_o).
+  rewrite (do_not_overlap_mload_aux' mem value' updates 26 offset offset' H_31_lt_32 H_o).
+  rewrite (do_not_overlap_mload_aux' mem value' updates 27 offset offset' H_31_lt_32 H_o).
+  rewrite (do_not_overlap_mload_aux' mem value' updates 28 offset offset' H_31_lt_32 H_o).
+  rewrite (do_not_overlap_mload_aux' mem value' updates 29 offset offset' H_31_lt_32 H_o).
+  rewrite (do_not_overlap_mload_aux' mem value' updates 30 offset offset' H_31_lt_32 H_o).
+  rewrite (do_not_overlap_mload_aux' mem value' updates 31 offset offset' H_31_lt_32 H_o).
+
+  assert ( H_O_0: (wordToN offset + 0 = wordToN offset)%N). apply N.add_0_r.
+  rewrite <- H_O_0.
+  rewrite (do_not_overlap_mload_aux' mem value' updates 0 offset offset' H_31_lt_32 H_o).
+  reflexivity.
+Qed.
+
+
+Lemma update_same_address_mstore'_aux:
+  forall n mem (value: word (n*8)) z offset1 offset2 x,
+    (x =? offset1)%N = false ->
+    (concrete_interpreter.ConcreteInterpreter.mstore' mem value offset2) x =
+      (concrete_interpreter.ConcreteInterpreter.mstore'
+         (fun (offset':N) => if (offset' =? offset1)%N then z else mem offset')
+         value
+         offset2) x.
+Proof. 
+  induction n as [|n' IHn'].
+  + intros.
+    simpl.
+    rewrite H.
+    reflexivity.
+  + intros.
+    simpl.
+    pose proof (IHn' mem (concrete_interpreter.ConcreteInterpreter.split2_byte value) z offset1 (offset2+1)%N x).
+    rewrite H0.
+    reflexivity.
+    apply H.
+Qed.
+
+Lemma update_same_address_mstore'_a:
+  forall n m mem (value: word (n*8)) (value' : word (m*8)) offset,
+    n>=m ->
+    concrete_interpreter.ConcreteInterpreter.mstore' mem value offset =
+      concrete_interpreter.ConcreteInterpreter.mstore' (concrete_interpreter.ConcreteInterpreter.mstore' mem value' offset) value offset.
+Proof.
+  induction n as [|n' IHn'].
+  + intros.
+    assert(m=0). intuition.
+    simpl.
+    unfold concrete_interpreter.ConcreteInterpreter.mstore'.
+    destruct m; try (discriminate || reflexivity).
+  + intros.
+    destruct m as [|m'] eqn:E_m.
+    ++ unfold concrete_interpreter.ConcreteInterpreter.mstore' at 3.
+       reflexivity.
+    ++ assert(n'>=m'). intuition.
+       pose proof (IHn' m' mem (concrete_interpreter.ConcreteInterpreter.split2_byte value) (concrete_interpreter.ConcreteInterpreter.split2_byte value') (offset+1)%N H0) as IHn'_0.
+       
+       apply functional_extensionality.
+       intro x.
+       simpl.
+       
+       destruct (x =? offset)%N eqn:E_x_offset; try reflexivity.
+       
+       pose proof (update_same_address_mstore'_aux n' (concrete_interpreter.ConcreteInterpreter.mstore' mem
+        (concrete_interpreter.ConcreteInterpreter.split2_byte value') (offset + 1)) (concrete_interpreter.ConcreteInterpreter.split2_byte value) (concrete_interpreter.ConcreteInterpreter.split1_byte value') offset (offset+1) x E_x_offset).
+       rewrite <- H1.
+       rewrite IHn'_0.
+       reflexivity.
+Qed.
+
+
+
+Lemma update_same_address_mstore':
+  forall n mem (value value': word (n*8)) offset, 
+    concrete_interpreter.ConcreteInterpreter.mstore' mem value offset =
+      concrete_interpreter.ConcreteInterpreter.mstore' (concrete_interpreter.ConcreteInterpreter.mstore' mem value' offset) value offset.
+Proof.
+  intros.
+  assert(H_ge_refl: n>=n). intuition.
+  pose proof (update_same_address_mstore'_a n n mem value value' offset H_ge_refl) as H_0.
+  apply H_0.
+Qed.  
+
+
+Lemma ge_Sn_Sm_ge_1:
+  forall n m,
+    S n > 0 -> S m < S n -> exists i, n = S i.
+Proof.
+  intros n m H1 H2.
+  destruct n as [|n'] eqn:E_n.
+  + apply lt_S_n in H2.
+    destruct m.
+    ++ apply Nat.lt_irrefl in H2. contradiction.
+    ++ apply Nat.nlt_0_r in H2. contradiction.     
+  + exists n'.
+    reflexivity.
+Qed.
+
+Lemma N_x_nat_of_Si:
+  forall x i,
+    (x + N.of_nat (S i) = x + 1 + N.of_nat i)%N.
+Proof.
+  intros x i.
+  rewrite Nat2N.inj_succ.
+  rewrite <- N.add_1_l.
+  repeat rewrite N.add_assoc.
+  reflexivity.
+Qed.
+
+
+
+Lemma update_same_address_mstore8_mstore':
+  forall i n mem (value : word (n*8)) (value': word (1*8)) offset,
+    n > 0 ->
+    i < n ->
+    concrete_interpreter.ConcreteInterpreter.mstore' mem value offset =
+      concrete_interpreter.ConcreteInterpreter.mstore' (concrete_interpreter.ConcreteInterpreter.mstore' mem value' (offset+ N.of_nat i)%N) value offset.
+Proof.
+  induction i as [|i' IHi'].
+  + intros n mem value value' offset H_n_gt_0 H_i_lt_n.
+    unfold  N.of_nat.
+    rewrite N.add_0_r.
+    apply update_same_address_mstore'_a.
+    intuition.
+  + destruct n as [|n'] eqn:E_n.
+    ++ intros mem value value' offset H_n_gt_0 H_i_l.
+       apply gt_irrefl in H_n_gt_0.
+       contradiction.
+    ++ intros mem value value' offset H_n_gt_0 H_i_lt_n.
+       pose proof (ge_Sn_Sm_ge_1 n' i' H_n_gt_0 H_i_lt_n) as H_n'_ge_1.
+       destruct H_n'_ge_1 as [n'' H_n'_ge_1].
+
+       rewrite N_x_nat_of_Si.
+
+       apply functional_extensionality.
+       intro x.
+       simpl.
+       destruct (x =? offset)%N eqn:E_x_offset; try reflexivity.
+
+
+       assert(H_n'_gt_0: n'>0). intuition.
+       assert(H_i'_lt_n': i'<n'). intuition.
+       pose proof (IHi' n' mem (concrete_interpreter.ConcreteInterpreter.split2_byte value) value' (offset+1)%N H_n'_gt_0 H_i'_lt_n') as IHi'_0.
+
+       rewrite IHi'_0.
+       simpl.
+       reflexivity.
+Qed.
+
+
+Lemma two_consecutive_updates_same_address_conc:
+  forall v v1 v2 mem mem',
+    eval_common.EvalCommon.update_memory mem (U_MSTORE EVMWord v v1 :: U_MSTORE EVMWord v v2 :: mem') = eval_common.EvalCommon.update_memory mem (U_MSTORE EVMWord v v1 :: mem').
+Proof.
+  intros v v1 v2 mem mem'.
+  simpl.
+  remember (eval_common.EvalCommon.update_memory mem mem') as mem_i.
+  
+  unfold concrete_interpreter.ConcreteInterpreter.mstore.
+  pose proof (update_same_address_mstore' 32 mem_i v1 v2 (wordToN v)).
+  symmetry in H.
+  rewrite H at 1.
+  reflexivity.
+Qed.
+
+Lemma two_consecutive_mstore8_updates_same_address_conc:
+  forall v v1 v2 mem mem',
+    eval_common.EvalCommon.update_memory mem (U_MSTORE8 EVMWord v v1 :: U_MSTORE8 EVMWord v v2 :: mem') = eval_common.EvalCommon.update_memory mem (U_MSTORE8 EVMWord v v1 :: mem').
+Proof.
+  intros v v1 v2 mem mem'.
+  simpl.
+  remember (eval_common.EvalCommon.update_memory mem mem') as mem_i.
+  
+  unfold concrete_interpreter.ConcreteInterpreter.mstore.
+  pose proof (update_same_address_mstore' 1 mem_i (concrete_interpreter.ConcreteInterpreter.split1_byte (v1 : word (BytesInEVMWord*8))) (concrete_interpreter.ConcreteInterpreter.split1_byte (v2 : word (BytesInEVMWord*8))) (wordToN v)).
+  symmetry in H.
+  rewrite H at 1.
+  reflexivity.
+Qed.
+
+
+Lemma inter_n_j:
+  forall n m j,
+    (n <=? m) && (m <=? n+j) = true ->
+    exists i, i <= j /\ (m = n+i).
+Proof.
+  intros n m j H.
+  exists (m-n).
+  apply andb_prop in H.
+  destruct H as [H1 H2].
+  rewrite Nat.leb_le in H1.
+  rewrite Nat.leb_le in H2.
+  split; try intuition.
+Qed.
+
+Lemma N_inter_n_j:
+  forall n m j,
+    ((n <=? m) && (m <=? n+ j) = true)%N ->
+    exists i, (i <= j)%N /\ (m = n+i)%N.
+Proof.
+  intros n m j H0.
+  apply andb_prop in H0.
+  destruct H0 as [H0_1 H0_2].
+  rewrite N.leb_le in H0_1.
+  rewrite N.leb_le in H0_2.
+  assert (H0_1_nat: N.to_nat n <= N.to_nat m). intuition.
+  assert (H0_2_nat: N.to_nat m <= N.to_nat n + N.to_nat j). intuition.
+  rewrite <- Nat.leb_le in H0_1_nat.
+  rewrite <- Nat.leb_le in H0_2_nat.
+  pose proof (conj H0_1_nat H0_2_nat) as H0_12.
+  apply andb_true_intro in H0_12.
+  pose proof (inter_n_j (N.to_nat n) (N.to_nat m) (N.to_nat j) H0_12) as H_nat.
+  destruct H_nat as [i [H_nat_1 H_nat_2]].
+  exists (N.of_nat i).
+  split.
+  + rewrite N.le_lteq.
+    apply Nat.le_lteq in H_nat_1.
+    destruct H_nat_1.
+    ++ left. apply Nlt_in. rewrite Nat2N.id.
+       apply H.
+    ++ right. rewrite H. rewrite N2Nat.id. reflexivity.
+  + pose proof N2Nat.inj.
+    apply N2Nat.inj.
+    rewrite N2Nat.inj_add.
+    rewrite Nat2N.id.
+    apply H_nat_2.
+Qed.
+  
+  
+  
+Lemma two_consecutive_updates_same_address_mstore8_conc:
+  forall offset offset_8 v1 v2 mem mem',
+    (wordToN offset <=? wordToN offset_8)%N && (wordToN offset_8 <=? wordToN offset + 31)%N = true ->
+    eval_common.EvalCommon.update_memory mem (U_MSTORE EVMWord offset v1 :: U_MSTORE8 EVMWord offset_8 v2 :: mem') = eval_common.EvalCommon.update_memory mem (U_MSTORE EVMWord offset v1 :: mem').
+Proof.
+  intros offset offset_8 v1 v2 mem mem' H.
+  simpl.
+  unfold concrete_interpreter.ConcreteInterpreter.mstore.
+  
+  pose proof (N_inter_n_j (wordToN offset) (wordToN offset_8) 31 H) as H_0.
+  destruct H_0 as [i [H_0_0 H_0_1]].
+  rewrite H_0_1.
+
+  assert(H_32: (N.to_nat 32%N = 32)). intuition.
+  assert(H1: BytesInEVMWord > 0). unfold BytesInEVMWord. intuition.
+  assert(H2: N.to_nat i < BytesInEVMWord).
+     unfold BytesInEVMWord.
+     rewrite <- H_32.
+     apply Nlt_out.
+     rewrite <- N.lt_succ_r in H_0_0.
+     simpl in H_0_0.
+     apply H_0_0.
+  
+  pose proof (update_same_address_mstore8_mstore' (N.to_nat i) BytesInEVMWord (eval_common.EvalCommon.update_memory mem mem') v1 (concrete_interpreter.ConcreteInterpreter.split1_byte (v2: word ((S (pred BytesInEVMWord))*8))) (wordToN offset) H1 H2) as H3.
+  rewrite N2Nat.id in H3.
+  rewrite H3.
+  reflexivity.
+Qed.
+                                               
+Lemma two_consecutive_updates_same_address:
+  forall ctx soffset soffset' svalue svalue' smem maxidx bs model mem strg exts ops v,
+    is_sat ctx ->
+    eval_sstack_val soffset model mem strg exts maxidx bs ops = Some v ->
+    eval_sstack_val soffset' model mem strg exts maxidx bs ops = Some v ->
+    valid_smemory maxidx smem ->
+    valid_bindings maxidx bs ops ->
+    valid_sstack_value maxidx soffset ->
+    valid_sstack_value maxidx svalue ->
+    valid_sstack_value maxidx soffset' ->
+    valid_sstack_value maxidx svalue' ->
+    is_model ctx model = true ->
+    eval_smemory (U_MSTORE sstack_val soffset svalue :: U_MSTORE sstack_val soffset' svalue' :: smem) maxidx bs model mem strg exts ops =
+      eval_smemory (U_MSTORE sstack_val soffset svalue :: smem) maxidx bs model mem strg exts ops.
+Proof.
+  intros ctx soffset soffset' svalue svalue' smem maxidx bs model mem strg exts ops v H_is_sat H_eval_soffset H_eval_soffset' H_valid_smem H_valid_bs H_valid_soffset H_valid_svalue H_vlaid_soffset' H_valid_svalue' H_is_model.
+
+  pose proof (eval_sstack_val'_succ (S maxidx) svalue model mem strg exts maxidx bs ops H_valid_svalue H_valid_bs (gt_Sn_n maxidx)) as H_eval_svalue.
+  destruct H_eval_svalue as [v1 H_eval_svalue].
+  pose proof (eval_sstack_val'_succ (S maxidx) svalue' model mem strg exts maxidx bs ops H_valid_svalue' H_valid_bs (gt_Sn_n maxidx)) as H_eval_svalue'.
+  destruct H_eval_svalue' as [v2 H_eval_svalue'].
+
+  unfold eval_smemory.
+  unfold eval_sstack_val.
+
+  assert( H_valid_u1_u2_smem: valid_smemory maxidx (U_MSTORE sstack_val soffset svalue :: U_MSTORE sstack_val soffset' svalue' :: smem)). simpl. auto.  
+  pose proof (H_map_o_smem ctx (S maxidx) model mem strg exts maxidx bs ops (U_MSTORE sstack_val soffset svalue :: U_MSTORE sstack_val soffset' svalue' :: smem) H_valid_u1_u2_smem H_valid_bs (gt_Sn_n maxidx) H_is_model) as H_map_o_smem_0.
+  destruct H_map_o_smem_0 as [u1_u2_smem_v H_map_o_smem_0].
+  rewrite H_map_o_smem_0.
+
+  assert( H_valid_u1_smem: valid_smemory maxidx (U_MSTORE sstack_val soffset svalue ::  smem)). simpl. auto.  
+  pose proof (H_map_o_smem ctx (S maxidx) model mem strg exts maxidx bs ops (U_MSTORE sstack_val soffset svalue :: smem) H_valid_u1_smem H_valid_bs (gt_Sn_n maxidx) H_is_model) as H_map_o_smem_1.
+  destruct H_map_o_smem_1 as [u1_smem_v H_map_o_smem_1].
+  rewrite H_map_o_smem_1.
+
+  pose proof (map_option_split_2 (memory_update sstack_val)  (memory_update EVMWord) (eval_common.EvalCommon.instantiate_memory_update (fun sv : sstack_val => eval_sstack_val' (S maxidx) sv model mem strg exts maxidx bs ops)) smem u1_u2_smem_v (U_MSTORE sstack_val soffset svalue) (U_MSTORE sstack_val soffset' svalue') H_map_o_smem_0) as H_map_o_smem_0_0.
+  destruct H_map_o_smem_0_0 as [u1_v [u2_v [smem_v [H_u1_u2_smem_v [H_map_o_smem_0_u1 [H_map_o_smem_0_u2 H_map_o_smem_0_smem]]]]]].
+
+  unfold eval_common.EvalCommon.instantiate_memory_update in H_map_o_smem_0_u1.
+  unfold eval_sstack_val in H_eval_soffset.
+  rewrite H_eval_soffset in H_map_o_smem_0_u1.
+  unfold eval_sstack_val in H_eval_svalue.
+  rewrite H_eval_svalue in H_map_o_smem_0_u1.
+  injection H_map_o_smem_0_u1 as H_map_o_smem_0_u1.
+
+  unfold eval_common.EvalCommon.instantiate_memory_update in H_map_o_smem_0_u2.
+  unfold eval_sstack_val in H_eval_soffset'.
+  rewrite H_eval_soffset' in H_map_o_smem_0_u2.
+  unfold eval_sstack_val in H_eval_svalue'.
+  rewrite H_eval_svalue' in H_map_o_smem_0_u2.
+  injection H_map_o_smem_0_u2 as H_map_o_smem_0_u2.
+  
+  pose proof (map_option_split (memory_update sstack_val)  (memory_update EVMWord) (eval_common.EvalCommon.instantiate_memory_update (fun sv : sstack_val => eval_sstack_val' (S maxidx) sv model mem strg exts maxidx bs ops)) smem u1_smem_v (U_MSTORE sstack_val soffset svalue) H_map_o_smem_1) as H_map_o_smem_1_0.
+  destruct H_map_o_smem_1_0 as [u1_v' [smem_v' [H_u1_smem_v' [H_map_o_smem_1_u1 H_map_o_smem_1_smem]]]].
+
+  unfold eval_common.EvalCommon.instantiate_memory_update in H_map_o_smem_1_u1.
+  rewrite H_eval_soffset in H_map_o_smem_1_u1.
+  rewrite H_eval_svalue in H_map_o_smem_1_u1.
+  injection H_map_o_smem_1_u1 as H_map_o_smem_1_u1.
+
+  rewrite H_u1_smem_v'. 
+  rewrite H_u1_u2_smem_v.
+  rewrite <- H_map_o_smem_0_u1.
+  rewrite <- H_map_o_smem_0_u2.
+  rewrite <- H_map_o_smem_1_u1.
+
+  rewrite H_map_o_smem_0_smem in H_map_o_smem_1_smem.
+  injection H_map_o_smem_1_smem as H_map_o_smem_1_smem.
+  rewrite <- H_map_o_smem_1_smem.
+
+  rewrite two_consecutive_updates_same_address_conc.
+  reflexivity.
+Qed.
+
+
+Lemma two_consecutive_mstore8_updates_same_address:
+  forall ctx soffset soffset' svalue svalue' smem maxidx bs model mem strg exts ops v,
+    is_sat ctx ->
+    eval_sstack_val soffset model mem strg exts maxidx bs ops = Some v ->
+    eval_sstack_val soffset' model mem strg exts maxidx bs ops = Some v ->
+    valid_smemory maxidx smem ->
+    valid_bindings maxidx bs ops ->
+    valid_sstack_value maxidx soffset ->
+    valid_sstack_value maxidx svalue ->
+    valid_sstack_value maxidx soffset' ->
+    valid_sstack_value maxidx svalue' ->
+    is_model ctx model = true ->
+    eval_smemory (U_MSTORE8 sstack_val soffset svalue :: U_MSTORE8 sstack_val soffset' svalue' :: smem) maxidx bs model mem strg exts ops =
+      eval_smemory (U_MSTORE8 sstack_val soffset svalue :: smem) maxidx bs model mem strg exts ops.
+Proof. 
+  intros ctx soffset soffset' svalue svalue' smem maxidx bs model mem strg exts ops v H_is_sat H_eval_soffset H_eval_soffset' H_valid_smem H_valid_bs H_valid_soffset H_valid_svalue H_vlaid_soffset' H_valid_svalue' H_is_model.
+
+  pose proof (eval_sstack_val'_succ (S maxidx) svalue model mem strg exts maxidx bs ops H_valid_svalue H_valid_bs (gt_Sn_n maxidx)) as H_eval_svalue.
+  destruct H_eval_svalue as [v1 H_eval_svalue].
+  pose proof (eval_sstack_val'_succ (S maxidx) svalue' model mem strg exts maxidx bs ops H_valid_svalue' H_valid_bs (gt_Sn_n maxidx)) as H_eval_svalue'.
+  destruct H_eval_svalue' as [v2 H_eval_svalue'].
+
+  unfold eval_smemory.
+  unfold eval_sstack_val.
+
+  assert( H_valid_u1_u2_smem: valid_smemory maxidx (U_MSTORE8 sstack_val soffset svalue :: U_MSTORE8 sstack_val soffset' svalue' :: smem)). simpl. auto.  
+  pose proof (H_map_o_smem ctx (S maxidx) model mem strg exts maxidx bs ops (U_MSTORE8 sstack_val soffset svalue :: U_MSTORE8 sstack_val soffset' svalue' :: smem) H_valid_u1_u2_smem H_valid_bs (gt_Sn_n maxidx) H_is_model) as H_map_o_smem_0.
+  destruct H_map_o_smem_0 as [u1_u2_smem_v H_map_o_smem_0].
+  rewrite H_map_o_smem_0.
+
+  assert( H_valid_u1_smem: valid_smemory maxidx (U_MSTORE8 sstack_val soffset svalue ::  smem)). simpl. auto.  
+  pose proof (H_map_o_smem ctx (S maxidx) model mem strg exts maxidx bs ops (U_MSTORE8 sstack_val soffset svalue :: smem) H_valid_u1_smem H_valid_bs (gt_Sn_n maxidx) H_is_model) as H_map_o_smem_1.
+  destruct H_map_o_smem_1 as [u1_smem_v H_map_o_smem_1].
+  rewrite H_map_o_smem_1.
+
+  pose proof (map_option_split_2 (memory_update sstack_val)  (memory_update EVMWord) (eval_common.EvalCommon.instantiate_memory_update (fun sv : sstack_val => eval_sstack_val' (S maxidx) sv model mem strg exts maxidx bs ops)) smem u1_u2_smem_v (U_MSTORE8 sstack_val soffset svalue) (U_MSTORE8 sstack_val soffset' svalue') H_map_o_smem_0) as H_map_o_smem_0_0.
+  destruct H_map_o_smem_0_0 as [u1_v [u2_v [smem_v [H_u1_u2_smem_v [H_map_o_smem_0_u1 [H_map_o_smem_0_u2 H_map_o_smem_0_smem]]]]]].
+
+  unfold eval_common.EvalCommon.instantiate_memory_update in H_map_o_smem_0_u1.
+  unfold eval_sstack_val in H_eval_soffset.
+  rewrite H_eval_soffset in H_map_o_smem_0_u1.
+  unfold eval_sstack_val in H_eval_svalue.
+  rewrite H_eval_svalue in H_map_o_smem_0_u1.
+  injection H_map_o_smem_0_u1 as H_map_o_smem_0_u1.
+
+  unfold eval_common.EvalCommon.instantiate_memory_update in H_map_o_smem_0_u2.
+  unfold eval_sstack_val in H_eval_soffset'.
+  rewrite H_eval_soffset' in H_map_o_smem_0_u2.
+  unfold eval_sstack_val in H_eval_svalue'.
+  rewrite H_eval_svalue' in H_map_o_smem_0_u2.
+  injection H_map_o_smem_0_u2 as H_map_o_smem_0_u2.
+  
+  pose proof (map_option_split (memory_update sstack_val)  (memory_update EVMWord) (eval_common.EvalCommon.instantiate_memory_update (fun sv : sstack_val => eval_sstack_val' (S maxidx) sv model mem strg exts maxidx bs ops)) smem u1_smem_v (U_MSTORE8 sstack_val soffset svalue) H_map_o_smem_1) as H_map_o_smem_1_0.
+  destruct H_map_o_smem_1_0 as [u1_v' [smem_v' [H_u1_smem_v' [H_map_o_smem_1_u1 H_map_o_smem_1_smem]]]].
+
+  unfold eval_common.EvalCommon.instantiate_memory_update in H_map_o_smem_1_u1.
+  rewrite H_eval_soffset in H_map_o_smem_1_u1.
+  rewrite H_eval_svalue in H_map_o_smem_1_u1.
+  injection H_map_o_smem_1_u1 as H_map_o_smem_1_u1.
+
+  rewrite H_u1_smem_v'. 
+  rewrite H_u1_u2_smem_v.
+  rewrite <- H_map_o_smem_0_u1.
+  rewrite <- H_map_o_smem_0_u2.
+  rewrite <- H_map_o_smem_1_u1.
+
+  rewrite H_map_o_smem_0_smem in H_map_o_smem_1_smem.
+  injection H_map_o_smem_1_smem as H_map_o_smem_1_smem.
+  rewrite <- H_map_o_smem_1_smem.
+
+  rewrite two_consecutive_mstore8_updates_same_address_conc.
+  reflexivity.
+Qed.
+
+
+Lemma two_consecutive_updates_same_address_mstore8:
+  forall ctx soffset soffset' svalue svalue' smem maxidx bs model mem strg exts ops v1 v2,
+    is_sat ctx ->
+    eval_sstack_val soffset model mem strg exts maxidx bs ops = Some v1 ->
+    eval_sstack_val soffset' model mem strg exts maxidx bs ops = Some v2 ->
+    valid_smemory maxidx smem ->
+    valid_bindings maxidx bs ops ->
+    valid_sstack_value maxidx soffset ->
+    valid_sstack_value maxidx svalue ->
+    valid_sstack_value maxidx soffset' ->
+    valid_sstack_value maxidx svalue' ->
+    is_model ctx model = true ->
+    andb ((wordToN v2) <=? (wordToN v1) )%N ((wordToN v1) <=? (wordToN v2)+31)%N = true ->
+    eval_smemory (U_MSTORE sstack_val soffset' svalue' :: U_MSTORE8 sstack_val soffset svalue :: smem) maxidx bs model mem strg exts ops =
+      eval_smemory (U_MSTORE sstack_val soffset' svalue' :: smem) maxidx bs model mem strg exts ops.
+Proof.
+  intros ctx soffset soffset' svalue svalue' smem maxidx bs model mem strg exts ops v1 v2 H_is_sat H_eval_soffset H_eval_soffset' H_valid_smem H_valid_bs H_valid_soffset H_valid_svalue H_vlaid_soffset' H_valid_svalue' H_is_model H_v1_in_v2.
+
+  pose proof (eval_sstack_val'_succ (S maxidx) svalue model mem strg exts maxidx bs ops H_valid_svalue H_valid_bs (gt_Sn_n maxidx)) as H_eval_svalue.
+  destruct H_eval_svalue as [svalue_v H_eval_svalue].
+  pose proof (eval_sstack_val'_succ (S maxidx) svalue' model mem strg exts maxidx bs ops H_valid_svalue' H_valid_bs (gt_Sn_n maxidx)) as H_eval_svalue'.
+  destruct H_eval_svalue' as [svalue'_v H_eval_svalue'].
+
+  unfold eval_smemory.
+  unfold eval_sstack_val.
+
+  assert( H_valid_u1_u2_smem: valid_smemory maxidx (U_MSTORE sstack_val soffset' svalue' :: U_MSTORE8 sstack_val soffset svalue :: smem)). simpl. auto.  
+  pose proof (H_map_o_smem ctx (S maxidx) model mem strg exts maxidx bs ops (U_MSTORE sstack_val soffset' svalue' :: U_MSTORE8 sstack_val soffset svalue :: smem) H_valid_u1_u2_smem H_valid_bs (gt_Sn_n maxidx) H_is_model) as H_map_o_smem_0.
+  destruct H_map_o_smem_0 as [u1_u2_smem_v H_map_o_smem_0].
+  rewrite H_map_o_smem_0.
+
+  assert( H_valid_u1_smem: valid_smemory maxidx (U_MSTORE sstack_val soffset' svalue' ::  smem)). simpl. auto.
+  pose proof (H_map_o_smem ctx (S maxidx) model mem strg exts maxidx bs ops (U_MSTORE sstack_val soffset' svalue' :: smem) H_valid_u1_smem H_valid_bs (gt_Sn_n maxidx) H_is_model) as H_map_o_smem_1.
+  destruct H_map_o_smem_1 as [u1_smem_v H_map_o_smem_1].
+  rewrite H_map_o_smem_1.
+
+  pose proof (map_option_split_2 (memory_update sstack_val)  (memory_update EVMWord) (eval_common.EvalCommon.instantiate_memory_update (fun sv : sstack_val => eval_sstack_val' (S maxidx) sv model mem strg exts maxidx bs ops)) smem u1_u2_smem_v (U_MSTORE sstack_val soffset' svalue') (U_MSTORE8 sstack_val soffset svalue) H_map_o_smem_0) as H_map_o_smem_0_0.
+  destruct H_map_o_smem_0_0 as [u1_v [u2_v [smem_v [H_u1_u2_smem_v [H_map_o_smem_0_u1 [H_map_o_smem_0_u2 H_map_o_smem_0_smem]]]]]].
+
+  unfold eval_common.EvalCommon.instantiate_memory_update in H_map_o_smem_0_u1.
+  unfold eval_sstack_val in H_eval_soffset'.
+  rewrite H_eval_soffset' in H_map_o_smem_0_u1.
+  unfold eval_sstack_val in H_eval_svalue'.
+  rewrite H_eval_svalue' in H_map_o_smem_0_u1.
+  injection H_map_o_smem_0_u1 as H_map_o_smem_0_u1.
+
+  unfold eval_common.EvalCommon.instantiate_memory_update in H_map_o_smem_0_u2.
+  unfold eval_sstack_val in H_eval_soffset.
+  rewrite H_eval_soffset in H_map_o_smem_0_u2.
+  unfold eval_sstack_val in H_eval_svalue.
+  rewrite H_eval_svalue in H_map_o_smem_0_u2.
+  injection H_map_o_smem_0_u2 as H_map_o_smem_0_u2.
+ 
+  pose proof (map_option_split (memory_update sstack_val)  (memory_update EVMWord) (eval_common.EvalCommon.instantiate_memory_update (fun sv : sstack_val => eval_sstack_val' (S maxidx) sv model mem strg exts maxidx bs ops)) smem u1_smem_v (U_MSTORE sstack_val soffset' svalue') H_map_o_smem_1) as H_map_o_smem_1_0.
+  destruct H_map_o_smem_1_0 as [u1_v' [smem_v' [H_u1_smem_v' [H_map_o_smem_1_u1 H_map_o_smem_1_smem]]]].
+
+  unfold eval_common.EvalCommon.instantiate_memory_update in H_map_o_smem_1_u1.
+  rewrite H_eval_soffset' in H_map_o_smem_1_u1.
+  rewrite H_eval_svalue' in H_map_o_smem_1_u1.
+  injection H_map_o_smem_1_u1 as H_map_o_smem_1_u1.
+
+  rewrite H_u1_smem_v'. 
+  rewrite H_u1_u2_smem_v.
+  rewrite <- H_map_o_smem_0_u1.
+  rewrite <- H_map_o_smem_0_u2.
+  rewrite <- H_map_o_smem_1_u1.
+ 
+  rewrite H_map_o_smem_0_smem in H_map_o_smem_1_smem.
+  injection H_map_o_smem_1_smem as H_map_o_smem_1_smem.
+  rewrite <- H_map_o_smem_1_smem.
+  rewrite two_consecutive_updates_same_address_mstore8_conc.
+  reflexivity.
+  apply H_v1_in_v2.
+Qed.
+
+
+Lemma mem_eq_after_update'':
+forall (n m : nat)  (mem1 mem2 : memory) (svalue1 : word (n * 8)) (svalue2 : word (m * 8)) (soffset1 soffset2 : N)  (w : N),
+  concrete_interpreter.ConcreteInterpreter.mstore' mem1 svalue1 soffset1 w =
+    concrete_interpreter.ConcreteInterpreter.mstore' mem2 svalue1 soffset1 w ->
+  concrete_interpreter.ConcreteInterpreter.mstore'
+    (concrete_interpreter.ConcreteInterpreter.mstore' mem1 svalue2 soffset2) svalue1 soffset1 w =
+  concrete_interpreter.ConcreteInterpreter.mstore'
+    (concrete_interpreter.ConcreteInterpreter.mstore' mem2 svalue2 soffset2) svalue1 soffset1 w.
+Proof.
+  induction n as [|n' IHn'].
+  + induction m as [|m' IHm'].
+    ++ intros mem1 mem2 svalue1 svalue2 soffset1 soffset2 w H.
+       unfold concrete_interpreter.ConcreteInterpreter.mstore' in H.
+       simpl.
+       apply H.
+    ++ intros mem1 mem2 svalue1 svalue2 soffset1 soffset2 w H.
+       simpl.
+       destruct (w =? soffset2)%N eqn:E_w_off2; try reflexivity.
+       pose proof (IHm' mem1 mem2 svalue1 (concrete_interpreter.ConcreteInterpreter.split2_byte svalue2) soffset1 (soffset2 + 1)%N w H) as IHm'_0.
+       simpl in IHm'_0.
+       apply IHm'_0.
+  +  intros m mem1 mem2 svalue1 svalue2 soffset1 soffset2 w H.
+     simpl.
+     destruct (w =? soffset1)%N eqn:E_w_off1; try reflexivity.
+     simpl in H.
+     rewrite E_w_off1 in H.
+     pose proof (IHn' m mem1 mem2 (concrete_interpreter.ConcreteInterpreter.split2_byte svalue1) svalue2 (soffset1+1)%N soffset2 w H).
+     apply H0.
+Qed.
+
+Lemma mem_eq_after_update':
+  forall u1 u2 w mem1 mem2,
+  (eval_common.EvalCommon.update_memory' mem1 u1) w =
+  (eval_common.EvalCommon.update_memory' mem2 u1) w ->
+  eval_common.EvalCommon.update_memory' (eval_common.EvalCommon.update_memory' mem1 u2) u1 w =
+  eval_common.EvalCommon.update_memory' (eval_common.EvalCommon.update_memory' mem2 u2) u1 w.
+Proof.
+  intros.
+  unfold eval_common.EvalCommon.update_memory'.
+  unfold eval_common.EvalCommon.update_memory'.
+  unfold concrete_interpreter.ConcreteInterpreter.mstore.
+   
+  destruct u1 as [soffset1 svalue1|soffset1 svalue1]; 
+    destruct u2 as [soffset2 svalue2|soffset2 svalue2]; 
+
+    apply mem_eq_after_update''; apply H.
+Qed.
+
+Lemma mem_eq_after_update:
+  forall smem1 smem2 u1 u2 w mem,
+  (eval_common.EvalCommon.update_memory' (eval_common.EvalCommon.update_memory mem smem1) u1) w =
+  (eval_common.EvalCommon.update_memory' (eval_common.EvalCommon.update_memory mem smem2) u1) w ->
+  eval_common.EvalCommon.update_memory' (eval_common.EvalCommon.update_memory' (eval_common.EvalCommon.update_memory mem smem1) u2) u1 w =
+  eval_common.EvalCommon.update_memory' (eval_common.EvalCommon.update_memory' (eval_common.EvalCommon.update_memory mem smem2) u2) u1 w.
+Proof.
+  intros.
+  pose proof (mem_eq_after_update' u1 u2 w (eval_common.EvalCommon.update_memory mem smem1) (eval_common.EvalCommon.update_memory mem smem2) H) as H_mem_eq_after_update'.
+  apply H_mem_eq_after_update'.
+Qed.
+
+Lemma N_of_nat_Sn:
+  forall x n, (x + N.of_nat (S n) = x+ 1 + N.of_nat n)%N.
+Proof.
+  intros x n.
+  apply N2Nat.inj_iff.
+  repeat rewrite N2Nat.inj_add.
+  intuition.
+Qed.
+
+
+Lemma mstore'_not_touched_addresses_remain_the_same:
+  forall sz mem w offset mem',
+    concrete_interpreter.ConcreteInterpreter.mstore' mem  (w : (word (sz*8))) offset = mem' ->
+    forall offset', (offset' >= offset + (N.of_nat sz))%N -> mem offset' = mem' offset'.
+Proof.
+  induction sz as [| sz' IHsz'].
+  + intros mem w n mem' H_mstore' n' H_n'_gt_n.
+    unfold concrete_interpreter.ConcreteInterpreter.mstore' in H_mstore'.
+    rewrite H_mstore'.
+    reflexivity.
+  + intros mem w offset mem' H_mstore' offset' H_n'_gt_n.
+    simpl in H_mstore'.
+    rewrite N_of_nat_Sn in H_n'_gt_n.
+    remember (concrete_interpreter.ConcreteInterpreter.mstore' mem (concrete_interpreter.ConcreteInterpreter.split2_byte w) (offset + 1)) as mem''.
+    pose proof (IHsz' mem (concrete_interpreter.ConcreteInterpreter.split2_byte w) (offset + 1)%N mem'' (eq_sym Heqmem'') offset' H_n'_gt_n) as IHsz'_0.
+    rewrite <- H_mstore'.
+    destruct (offset' =? offset)%N eqn:E_offset_offset'.
+    ++ rewrite N.eqb_eq in E_offset_offset'.
+       rewrite E_offset_offset' in H_n'_gt_n.
+       contradiction H_n'_gt_n.
+       destruct offset.
+       +++ intuition.
+       +++ intuition.
+    ++ rewrite IHsz'_0.
+       reflexivity.
+Qed.
+
+Lemma basic_mload_solver_snd: mload_solver_ext_snd basic_mload_solver.
+  unfold mload_solver_ext_snd.
+  unfold mload_solver_snd.
+  intros sstack_val_cmp H_sstack_val_cmp.
+  split. apply basic_mload_solver_valid.
+  unfold mload_solver_correct_res.
+  intros ctx m smem soffset smv ops idx1 m1.
+  intros H_is_sat H_valid_smap H_valid_smem H_valid_soffset H_basic_mload_solver H_add_to_smap.
+  induction smem as [|u smem' IHsmem'].
+  + exists idx1. exists m1.
+    split.
+    ++ simpl in H_basic_mload_solver.
+       rewrite <- H_basic_mload_solver in H_add_to_smap.
+       apply H_add_to_smap.
+    ++ intros model mem strg exts H_stk_len.
+       simpl in H_basic_mload_solver.
+       rewrite <- H_basic_mload_solver in H_add_to_smap.
+       destruct m as [maxidx bs] eqn:E_m.
+       simpl in H_add_to_smap.
+       injection H_add_to_smap as H_idx1 H_m1.
+       rewrite <- H_m1.
+       rewrite <- H_idx1.
+       simpl.
+       unfold eval_sstack_val.
+       remember (S maxidx) as S_maxidx.
+       unfold eval_sstack_val'.
+       fold eval_sstack_val'.
+       unfold follow_in_smap.
+       fold follow_in_smap.
+       rewrite Nat.eqb_refl.
+       simpl.
+       
+       assert(H_S_S_maxid_gt_maxidx: (S (S maxidx) > maxidx)). auto.
+       pose proof (eval_sstack_val'_succ (S maxidx) soffset model mem strg exts maxidx bs ops H_valid_soffset H_valid_smap (gt_Sn_n maxidx)) as H_eval_soffset.
+       destruct H_eval_soffset as [soffset_v H_eval_soffset].
+       rewrite HeqS_maxidx.
+       rewrite H_eval_soffset.
+       exists (concrete_interpreter.ConcreteInterpreter.mload mem soffset_v).
+       split; reflexivity.
+  + unfold basic_mload_solver in H_basic_mload_solver.
+    fold basic_mload_solver in H_basic_mload_solver.
+    destruct u as [soffset' svalue | soffset' svalue] eqn:E_u.
+    ++ destruct (sstack_val_cmp (S (get_maxidx_smap m)) ctx soffset soffset' (get_maxidx_smap m) (get_bindings_smap m) (get_maxidx_smap m) (get_bindings_smap m) ops) eqn:E_cmp_soffset_soffset'.
+       +++ rewrite <- H_basic_mload_solver in H_add_to_smap.
+           destruct m as [maxidx bs] eqn:E_m.
+           simpl in H_add_to_smap.
+             injection H_add_to_smap as H_idx1 H_m1.
+             rewrite <- H_idx1.
+             rewrite <- H_m1.
+             simpl.
+             exists maxidx.
+             exists (SymMap (S maxidx) ((maxidx, SymMLOAD soffset (U_MSTORE sstack_val soffset' svalue :: smem')) :: bs)).
+             split; try reflexivity.
+             intros model mem strg exts H_is_model.
+             simpl.
+             unfold eval_sstack_val.
+             
+             pose proof (eval_sstack_val'_immediate_fresh_var (S (S maxidx)) maxidx model mem strg exts svalue bs ops) as H_eval_fresh_maxidx_0.
+             rewrite  H_eval_fresh_maxidx_0.
+
+             simpl in H_valid_smem.
+             destruct H_valid_smem as [[H_valid_soffset' H_valid_svalue] H_valid_smem'].
+
+             pose proof (eval_sstack_val'_succ (S maxidx) svalue model mem strg exts maxidx bs ops H_valid_svalue H_valid_smap (gt_Sn_n maxidx)) as H_eval_svalue.
+             destruct H_eval_svalue as [svalue_v H_eval_svalue].
+             
+             pose proof (eval_sstack_val'_preserved_when_depth_extended (S maxidx) maxidx bs svalue svalue_v model mem strg exts ops H_eval_svalue) as H_eval_svalue_bis.
+             
+             exists svalue_v.
+             split. apply H_eval_svalue_bis.
+             remember (S maxidx) as S_maxidx.
+             unfold eval_sstack_val'.
+             fold eval_sstack_val'.
+             unfold follow_in_smap.
+             rewrite Nat.eqb_refl.
+             simpl.
+             rewrite HeqS_maxidx.
+             pose proof (eval_sstack_val'_succ (S maxidx) soffset' model mem strg exts maxidx bs ops H_valid_soffset' H_valid_smap (gt_Sn_n maxidx)) as H_eval_soffset'.
+             destruct  H_eval_soffset' as [soffset'_v H_eval_soffset'].
+             rewrite H_eval_soffset'.
+             rewrite HeqS_maxidx in  H_eval_svalue.
+             rewrite H_eval_svalue.
+             pose proof (H_map_o_smem ctx (S maxidx) model mem strg exts maxidx bs ops smem' H_valid_smem' H_valid_smap (gt_Sn_n maxidx) H_is_model) as H_mo_1.
+             destruct H_mo_1 as [v H_mo_1].
+             rewrite H_mo_1.
+             pose proof (eval_sstack_val'_succ (S maxidx) soffset model mem strg exts maxidx bs ops H_valid_soffset H_valid_smap (gt_Sn_n maxidx)) as H_eval_soffset.
+             destruct H_eval_soffset as [soffset_v H_eval_soffset].
+             rewrite H_eval_soffset.
+             simpl.
+             simpl in E_cmp_soffset_soffset'.
+             unfold safe_sstack_val_cmp_ext_1 in H_sstack_val_cmp.
+             unfold safe_sstack_val_cmp_ext_1_d in H_sstack_val_cmp.
+             unfold safe_sstack_val_cmp in H_sstack_val_cmp.
+             pose proof (H_sstack_val_cmp (S maxidx) (S maxidx) (Nat.le_refl (S maxidx)) ctx soffset soffset' maxidx bs maxidx bs ops H_is_sat H_valid_soffset H_valid_soffset' H_valid_smap H_valid_smap E_cmp_soffset_soffset' model mem strg exts H_is_model) as H_eval_soffset_soffset'.
+             unfold eval_sstack_val in H_eval_soffset_soffset'.
+             destruct  H_eval_soffset_soffset' as [soffset_soffset'_v  [H_eval_soffset_bis  H_eval_soffset'_bis]].
+             rewrite H_eval_soffset' in H_eval_soffset'_bis.
+             injection H_eval_soffset'_bis as H_eval_soffset'_bis.
+             rewrite H_eval_soffset in H_eval_soffset_bis.
+             injection H_eval_soffset_bis as H_eval_soffset_bis.           
+             rewrite H_eval_soffset'_bis.
+             rewrite H_eval_soffset_bis.
+             pose proof (mload_mstore_same_address (eval_common.EvalCommon.update_memory mem v) soffset_soffset'_v svalue_v) as H_mload_mstore_same_address.
+             rewrite H_mload_mstore_same_address.
+             reflexivity.
+       +++ destruct (memory_slots_do_not_overlap ctx soffset soffset' 31 31) eqn:E_not_overlap.
+           ++++ destruct m as [maxidx sb] eqn:E_m.
+                simpl in H_valid_smem.
+                destruct H_valid_smem as [[H_valid_soffset' H_valid_svalue] H_valid_smem'].
+
+                simpl.
+                exists maxidx.
+                exists (SymMap (S maxidx) ((maxidx, SymMLOAD soffset (U_MSTORE sstack_val soffset' svalue :: smem')) :: sb)).
+                split; try reflexivity.
+
+                intros model mem strg exts H_is_model.
+
+                pose proof (IHsmem' H_valid_smem' H_basic_mload_solver) as IHsmem'_0.
+                destruct IHsmem'_0 as [idx2 [m2 [H_add_to_smap' IHsmem'_0]]].
+                pose proof (IHsmem'_0 model mem strg exts H_is_model) as IHsmem'_1.
+                destruct IHsmem'_1 as [v' [H_eval_freshvar_idx1 H_eval_fresh_var_maxidx]].
+                exists v'.
+                split; auto.
+                simpl.
+
+                unfold eval_sstack_val.
+                remember (S maxidx) as S_maxidx.
+                unfold eval_sstack_val'.
+                fold eval_sstack_val'.
+                unfold follow_in_smap.
+                rewrite Nat.eqb_refl.
+                simpl.
+ 
+                pose proof (H_memory_slots_do_not_overlap ctx soffset soffset' 31 31 maxidx sb ops H_valid_smap H_valid_soffset H_valid_soffset' E_not_overlap model mem strg exts H_is_model) as H_memory_slots_do_not_overlap_0.
+                destruct H_memory_slots_do_not_overlap_0 as [v1' [v2' [H_eval_soffset_bis [H_eval_soffset' H_not_overlap]]]].
+                rewrite HeqS_maxidx.
+                
+                rewrite H_eval_soffset'.
+                pose proof (eval_sstack_val'_succ (S maxidx) svalue model mem strg exts maxidx sb ops H_valid_svalue H_valid_smap (gt_Sn_n maxidx)) as H_eval_svalue.
+                destruct H_eval_svalue as [svalue_v H_eval_svalue].
+                rewrite H_eval_svalue.
+
+                pose proof (H_map_o_smem ctx (S maxidx) model mem strg exts maxidx sb ops smem' H_valid_smem' H_valid_smap (gt_Sn_n maxidx) H_is_model) as H_mo_1.
+                destruct H_mo_1 as [v''' H_mo_1].
+                rewrite H_mo_1.
+                
+                rewrite H_eval_soffset_bis.
+
+                unfold concrete_interpreter.ConcreteInterpreter.mload.
+                unfold concrete_interpreter.ConcreteInterpreter.mload'.
+
+                pose proof (do_not_overlap_mload mem v1' v2' svalue_v v''' H_not_overlap) as H_do_not_overlap_mload.
+                rewrite H_do_not_overlap_mload.
+                
+                simpl in H_add_to_smap'.
+                injection H_add_to_smap' as H_idx2 H_m2.
+                rewrite <- H_m2 in H_eval_fresh_var_maxidx.
+                rewrite <- H_idx2 in H_eval_fresh_var_maxidx.
+                simpl in H_eval_fresh_var_maxidx.
+
+                unfold eval_sstack_val in H_eval_fresh_var_maxidx.
+                rewrite <- HeqS_maxidx in H_eval_fresh_var_maxidx.
+                unfold eval_sstack_val' in H_eval_fresh_var_maxidx.
+                fold eval_sstack_val' in H_eval_fresh_var_maxidx.
+                unfold follow_in_smap in H_eval_fresh_var_maxidx.
+                rewrite Nat.eqb_refl in H_eval_fresh_var_maxidx.
+                simpl in H_eval_fresh_var_maxidx.
+                destruct (map_option (eval_common.EvalCommon.instantiate_memory_update (fun sv : sstack_val => eval_sstack_val' S_maxidx sv model mem strg exts maxidx sb ops)) smem') as [smem_updates|] eqn:E_mo_1; try discriminate.
+                
+                
+                rewrite HeqS_maxidx in H_eval_fresh_var_maxidx.
+                rewrite H_eval_soffset_bis in H_eval_fresh_var_maxidx.
+                injection H_eval_fresh_var_maxidx as H_v'.
+                unfold concrete_interpreter.ConcreteInterpreter.mload in H_v'.
+                unfold concrete_interpreter.ConcreteInterpreter.mload' in H_v'.
+                rewrite HeqS_maxidx in E_mo_1.
+                rewrite E_mo_1 in H_mo_1.
+                injection H_mo_1 as H_mo_1.
+                rewrite <- H_mo_1.
+                rewrite <- H_v'.
+                reflexivity.
+           ++++ destruct m as [maxidx sb] eqn:E_m. 
+                simpl.
+                exists maxidx.
+                exists (SymMap (S maxidx) ((maxidx, SymMLOAD soffset (U_MSTORE sstack_val soffset' svalue :: smem')) :: sb)).
+                split; try reflexivity.
+                intros model mem strg exts.
+                intros H_id_model.
+                simpl.
+                rewrite <- H_basic_mload_solver in H_add_to_smap.
+                simpl in H_add_to_smap.
+                injection H_add_to_smap as H_idx1 H_m1.
+                rewrite <- H_m1.
+                simpl.
+                rewrite <- H_idx1.
+                
+                unfold eval_sstack_val.
+                remember (S maxidx) as S_maxidx.
+
+                assert(H_valid_freshvar_maxidx: valid_sstack_value S_maxidx (FreshVar maxidx)).
+                  (* proof of assert *)
+                   simpl.
+                   rewrite HeqS_maxidx.
+                   apply lt_n_Sn.
+
+               assert(H_valid_ex_bs: valid_bindings S_maxidx ((maxidx, SymMLOAD soffset (U_MSTORE sstack_val soffset' svalue :: smem')) :: sb) ops).
+                   (* proof of assert *)
+                   rewrite HeqS_maxidx.
+                   simpl.
+                   split; try auto.
+                   
+                
+                   pose proof (eval_sstack_val'_succ (S S_maxidx) (FreshVar maxidx) model mem strg exts S_maxidx ((maxidx, SymMLOAD soffset (U_MSTORE sstack_val soffset' svalue :: smem')) :: sb) ops H_valid_freshvar_maxidx H_valid_ex_bs (gt_Sn_n S_maxidx)) as H_eval_freshvar_maxidx.
+                   destruct H_eval_freshvar_maxidx as [v H_eval_freshvar_maxidx].
+                   exists v.
+                   split; apply H_eval_freshvar_maxidx.
+                    
+    (* MSTIRE8 -- copy of the previous one with changes that replace MSTORE by MSTORE8*)
+    ++ destruct (memory_slots_do_not_overlap ctx soffset soffset' 31 0) eqn:E_not_overlap.
+       +++ destruct m as [maxidx sb] eqn:E_m.
+          simpl in H_valid_smem.
+          destruct H_valid_smem as [[H_valid_soffset' H_valid_svalue] H_valid_smem'].
+
+          simpl.
+          exists maxidx.
+          exists (SymMap (S maxidx) ((maxidx, SymMLOAD soffset (U_MSTORE8 sstack_val soffset' svalue :: smem')) :: sb)).
+          split; try reflexivity.
+
+          intros model mem strg exts H_is_model.
+
+          pose proof (IHsmem' H_valid_smem' H_basic_mload_solver) as IHsmem'_0.
+          destruct IHsmem'_0 as [idx2 [m2 [H_add_to_smap' IHsmem'_0]]].
+          pose proof (IHsmem'_0 model mem strg exts H_is_model) as IHsmem'_1.
+          destruct IHsmem'_1 as [v' [H_eval_freshvar_idx1 H_eval_fresh_var_maxidx]].
+          exists v'.
+          split; auto.
+          simpl.
+
+          unfold eval_sstack_val.
+          remember (S maxidx) as S_maxidx.
+          unfold eval_sstack_val'.
+          fold eval_sstack_val'.
+          unfold follow_in_smap.
+          rewrite Nat.eqb_refl.
+          simpl.
+ 
+          pose proof (H_memory_slots_do_not_overlap ctx soffset soffset' 31 0 maxidx sb ops H_valid_smap H_valid_soffset H_valid_soffset' E_not_overlap model mem strg exts H_is_model) as H_memory_slots_do_not_overlap_0.
+          destruct H_memory_slots_do_not_overlap_0 as [v1' [v2' [H_eval_soffset_bis [H_eval_soffset' H_not_overlap]]]].
+          rewrite HeqS_maxidx.
+                
+          rewrite H_eval_soffset'.
+          pose proof (eval_sstack_val'_succ (S maxidx) svalue model mem strg exts maxidx sb ops H_valid_svalue H_valid_smap (gt_Sn_n maxidx)) as H_eval_svalue.
+          destruct H_eval_svalue as [svalue_v H_eval_svalue].
+          rewrite H_eval_svalue.
+          
+          pose proof (H_map_o_smem ctx (S maxidx) model mem strg exts maxidx sb ops smem' H_valid_smem' H_valid_smap (gt_Sn_n maxidx) H_is_model) as H_mo_1.
+          destruct H_mo_1 as [v''' H_mo_1].
+          rewrite H_mo_1.
+                
+          rewrite H_eval_soffset_bis.
+
+          unfold concrete_interpreter.ConcreteInterpreter.mload.
+          unfold concrete_interpreter.ConcreteInterpreter.mload'.
+
+          pose proof (do_not_overlap_mload_0 mem v1' v2' svalue_v v''' H_not_overlap) as H_do_not_overlap_mload.
+          rewrite H_do_not_overlap_mload.
+                
+          simpl in H_add_to_smap'.
+          injection H_add_to_smap' as H_idx2 H_m2.
+          rewrite <- H_m2 in H_eval_fresh_var_maxidx.
+          rewrite <- H_idx2 in H_eval_fresh_var_maxidx.
+          simpl in H_eval_fresh_var_maxidx.
+
+          unfold eval_sstack_val in H_eval_fresh_var_maxidx.
+          rewrite <- HeqS_maxidx in H_eval_fresh_var_maxidx.
+          unfold eval_sstack_val' in H_eval_fresh_var_maxidx.
+          fold eval_sstack_val' in H_eval_fresh_var_maxidx.
+          unfold follow_in_smap in H_eval_fresh_var_maxidx.
+          rewrite Nat.eqb_refl in H_eval_fresh_var_maxidx.
+          simpl in H_eval_fresh_var_maxidx.
+          destruct (map_option (eval_common.EvalCommon.instantiate_memory_update (fun sv : sstack_val => eval_sstack_val' S_maxidx sv model mem strg exts maxidx sb ops)) smem') as [smem_updates|] eqn:E_mo_1; try discriminate.
+                
+                
+          rewrite HeqS_maxidx in H_eval_fresh_var_maxidx.
+          rewrite H_eval_soffset_bis in H_eval_fresh_var_maxidx.
+          injection H_eval_fresh_var_maxidx as H_v'.
+          unfold concrete_interpreter.ConcreteInterpreter.mload in H_v'.
+          unfold concrete_interpreter.ConcreteInterpreter.mload' in H_v'.
+          rewrite HeqS_maxidx in E_mo_1.
+          rewrite E_mo_1 in H_mo_1.
+          injection H_mo_1 as H_mo_1.
+          rewrite <- H_mo_1.
+          rewrite <- H_v'.
+          reflexivity.
+       +++ destruct m as [maxidx sb] eqn:E_m. 
+           simpl.
+           exists maxidx.
+           exists (SymMap (S maxidx) ((maxidx, SymMLOAD soffset (U_MSTORE8 sstack_val soffset' svalue :: smem')) :: sb)).
+           split; try reflexivity.
+           intros model mem strg exts.
+           intros H_is_model.
+           simpl.
+           rewrite <- H_basic_mload_solver in H_add_to_smap.
+           simpl in H_add_to_smap.
+           injection H_add_to_smap as H_idx1 H_m1.
+           rewrite <- H_m1.
+           simpl.
+           rewrite <- H_idx1.
+                
+           unfold eval_sstack_val.
+           remember (S maxidx) as S_maxidx.
+
+           assert(H_valid_freshvar_maxidx: valid_sstack_value S_maxidx (FreshVar maxidx)).
+             (* proof of assert *)
+             simpl.
+             rewrite HeqS_maxidx.
+             apply lt_n_Sn.
+
+          assert(H_valid_ex_bs: valid_bindings S_maxidx ((maxidx, SymMLOAD soffset (U_MSTORE8 sstack_val soffset' svalue :: smem')) :: sb) ops).
+            (* proof of assert *)
+            rewrite HeqS_maxidx.
+            simpl.
+            split; try auto.
+                   
+                
+            pose proof (eval_sstack_val'_succ (S S_maxidx) (FreshVar maxidx) model mem strg exts S_maxidx ((maxidx, SymMLOAD soffset (U_MSTORE8 sstack_val soffset' svalue :: smem')) :: sb) ops H_valid_freshvar_maxidx H_valid_ex_bs (gt_Sn_n S_maxidx)) as H_eval_freshvar_maxidx.
+            destruct H_eval_freshvar_maxidx as [v H_eval_freshvar_maxidx].
+            exists v.
+            split; apply H_eval_freshvar_maxidx.
+Qed.
+
+
+  Lemma basic_smemory_updater_remove_mstore_dups_valid:
+    forall sstack_val_cmp ctx soffset m ops smem smem_r,
+      is_sat ctx ->
+      symbolic_state_cmp.SymbolicStateCmp.safe_sstack_val_cmp_ext_1 sstack_val_cmp ->
+      valid_sstack_value (get_maxidx_smap m) soffset ->
+      valid_smemory (get_maxidx_smap m) smem ->
+      basic_smemory_updater_remove_mstore_dups sstack_val_cmp ctx soffset smem m ops = smem_r ->
+      valid_smemory (get_maxidx_smap m) smem_r.
+  Proof.
+    intros sstack_val_cmp ctx soffset m ops.
+    induction smem as [| u smem' IHsmem'].
+    + intros smem_r H_is_sat H_sstack_val_cmp_snd H_valid_soffset H_valid_smem H_basic_smem_updater_remove_dups.
+      simpl in H_basic_smem_updater_remove_dups.
+      rewrite <- H_basic_smem_updater_remove_dups.
+      reflexivity.
+    + intros smem_r H_is_sat H_sstack_val_cmp_snd H_valid_soffset H_valid_smem H_basic_smem_updater_remove_dups.
+      unfold basic_smemory_updater_remove_mstore_dups in H_basic_smem_updater_remove_dups.
+      fold basic_smemory_updater_remove_mstore_dups in H_basic_smem_updater_remove_dups.
+      destruct u as [soffset' svalue|soffset' svalue] eqn:E_u.
+      ++ destruct (sstack_val_cmp (S (get_maxidx_smap m)) ctx soffset soffset' (get_maxidx_smap m) (get_bindings_smap m) (get_maxidx_smap m) (get_bindings_smap m) ops) eqn:E_cmp_soffset_soffset'.
+         +++ apply IHsmem'.
+             ++++ apply H_is_sat.
+             ++++ apply H_sstack_val_cmp_snd.
+             ++++ apply H_valid_soffset.
+             ++++ apply H_valid_smem.
+             ++++ apply H_basic_smem_updater_remove_dups.
+         +++ destruct smem_r as [|u_r smem_r']; try discriminate.
+             injection H_basic_smem_updater_remove_dups as H_u_r H_smem_r'.
+             simpl.
+             split.
+             ++++ rewrite <- H_u_r.
+                  simpl.
+                  split; apply H_valid_smem.
+             ++++ apply IHsmem'.
+                  +++++ apply H_is_sat.
+                  +++++ apply H_sstack_val_cmp_snd.
+                  +++++ apply H_valid_soffset.
+                  +++++ apply H_valid_smem.
+                  +++++ apply H_smem_r'.
+      ++ destruct (mstore8_is_included_in_mstore sstack_val_cmp ctx soffset' soffset) eqn:E_cmp_soffset_soffset'.
+         +++ apply IHsmem'.
+             ++++ apply H_is_sat.
+             ++++ apply H_sstack_val_cmp_snd.
+             ++++ apply H_valid_soffset.
+             ++++ apply H_valid_smem.
+             ++++ apply H_basic_smem_updater_remove_dups.
+         +++ destruct smem_r as [|u_r smem_r']; try discriminate.
+             injection H_basic_smem_updater_remove_dups as H_u_r H_smem_r'.
+             simpl.
+             split.
+             ++++ rewrite <- H_u_r.
+                  simpl.
+                  split; apply H_valid_smem.
+             ++++ apply IHsmem'.
+                  +++++ apply H_is_sat.
+                  +++++ apply H_sstack_val_cmp_snd.
+                  +++++ apply H_valid_soffset.
+                  +++++ apply H_valid_smem.
+                  +++++ apply H_smem_r'.
+  Qed.
+
+    Lemma basic_smemory_updater_remove_mstore8_dups_valid:
+    forall sstack_val_cmp ctx soffset m ops smem smem_r,
+      is_sat ctx ->
+      symbolic_state_cmp.SymbolicStateCmp.safe_sstack_val_cmp_ext_1 sstack_val_cmp ->
+      valid_sstack_value (get_maxidx_smap m) soffset ->
+      valid_smemory (get_maxidx_smap m) smem ->
+      basic_smemory_updater_remove_mstore8_dups sstack_val_cmp ctx soffset smem m ops = smem_r ->
+      valid_smemory (get_maxidx_smap m) smem_r.
+  Proof.
+    intros sstack_val_cmp ctx soffset m ops.
+    induction smem as [| u smem' IHsmem'].
+    + intros smem_r H_is_sat H_sstack_val_cmp_snd H_valid_soffset H_valid_smem H_basic_smem_updater_remove_dups.
+      simpl in H_basic_smem_updater_remove_dups.
+      rewrite <- H_basic_smem_updater_remove_dups.
+      reflexivity.
+    + intros smem_r H_is_sat H_sstack_val_cmp_snd H_valid_soffset H_valid_smem H_basic_smem_updater_remove_dups.
+      unfold basic_smemory_updater_remove_mstore8_dups in H_basic_smem_updater_remove_dups.
+      fold basic_smemory_updater_remove_mstore8_dups in H_basic_smem_updater_remove_dups.
+      destruct u as [soffset' svalue|soffset' svalue] eqn:E_u.
+      ++ destruct smem_r as [|u_r smem_r']; try discriminate.
+         injection H_basic_smem_updater_remove_dups as H_u_r H_smem_r'.
+         simpl.
+         split.
+         +++ rewrite <- H_u_r.
+             simpl.
+             split; apply H_valid_smem.
+         +++ apply IHsmem'.
+             ++++ apply H_is_sat.
+             ++++ apply H_sstack_val_cmp_snd.
+             ++++ apply H_valid_soffset.
+             ++++ apply H_valid_smem.
+             ++++ apply H_smem_r'.
+
+      ++ destruct (sstack_val_cmp (S (get_maxidx_smap m)) ctx soffset soffset' (get_maxidx_smap m) (get_bindings_smap m) (get_maxidx_smap m) (get_bindings_smap m) ops) eqn:E_cmp_soffset_soffset'.
+         +++ apply IHsmem'.
+             ++++ apply H_is_sat.
+             ++++ apply H_sstack_val_cmp_snd.
+             ++++ apply H_valid_soffset.
+             ++++ apply H_valid_smem.
+             ++++ apply H_basic_smem_updater_remove_dups.
+         +++ destruct smem_r as [|u_r smem_r']; try discriminate.
+             injection H_basic_smem_updater_remove_dups as H_u_r H_smem_r'.
+             simpl.
+             split.
+             ++++ rewrite <- H_u_r.
+                  simpl.
+                  split; apply H_valid_smem.
+             ++++ apply IHsmem'.
+                  +++++ apply H_is_sat.
+                  +++++ apply H_sstack_val_cmp_snd.
+                  +++++ apply H_valid_soffset.
+                  +++++ apply H_valid_smem.
+                  +++++ apply H_smem_r'.
+  Qed.
+
+  Lemma basic_smemory_updater_valid: 
+    forall sstack_val_cmp : symbolic_state_cmp.SymbolicStateCmp.sstack_val_cmp_ext_1_t,
+      symbolic_state_cmp.SymbolicStateCmp.safe_sstack_val_cmp_ext_1 sstack_val_cmp ->
+      smemory_updater_valid_res (basic_smemory_updater sstack_val_cmp).
+  Proof.
+    intros sstack_val_cmp H_sstack_val_cmp_snd.
+    unfold smemory_updater_valid_res.
+    intros ctx m smem smem' u ops.
+    intros H_is_sat H_valid_smem H_valid_u H_basic_smem_updater.
+    unfold basic_smemory_updater in H_basic_smem_updater.
+    destruct u as [soffset svalue|soffset svalue] eqn:E_u.
+    + destruct smem' as [|u' smem'']; try discriminate.
+      injection H_basic_smem_updater as H_u' H_smem''.
+      rewrite <- H_u'.
+      simpl.
+      split; try split; try apply H_valid_u.
+      apply basic_smemory_updater_remove_mstore_dups_valid in H_smem''.
+    
+      ++ apply H_smem''.
+      ++ apply H_is_sat.
+      ++ apply H_sstack_val_cmp_snd.
+      ++ apply H_valid_u.
+      ++ apply H_valid_smem.
+    + destruct smem' as [|u' smem'']; try discriminate.
+      injection H_basic_smem_updater as H_u' H_smem''.
+      rewrite <- H_u'.
+      simpl.
+      split; try split; try apply H_valid_u.
+      apply basic_smemory_updater_remove_mstore8_dups_valid in H_smem''.
+    
+      ++ apply H_smem''.
+      ++ apply H_is_sat.
+      ++ apply H_sstack_val_cmp_snd.
+      ++ apply H_valid_u.
+      ++ apply H_valid_smem.
+   Qed. 
+
+
+  
+  Lemma basic_smemory_updater_remove_dups_correct_eq_key:
+    forall sstack_val_cmp ctx soffset svalue model mem strg exts m ops smem1 smem2 mem1 mem2 v,
+      symbolic_state_cmp.SymbolicStateCmp.safe_sstack_val_cmp_ext_1 sstack_val_cmp ->
+      is_sat ctx ->
+      is_model ctx model = true ->
+      valid_sstack_value (get_maxidx_smap m) soffset ->
+      valid_sstack_value (get_maxidx_smap m) svalue ->
+      valid_smap (get_maxidx_smap m) (get_bindings_smap m) ops ->
+      valid_smemory (get_maxidx_smap m) smem1 ->
+      valid_smemory (get_maxidx_smap m) smem2 ->
+      eval_smemory (U_MSTORE sstack_val soffset svalue :: smem1) (get_maxidx_smap m) (get_bindings_smap m) model mem strg exts ops = Some mem1 ->
+      eval_smemory (U_MSTORE sstack_val soffset svalue :: smem2) (get_maxidx_smap m) (get_bindings_smap m) model mem strg exts ops = Some mem2 ->
+      eval_sstack_val' (S (get_maxidx_smap m)) soffset model mem strg exts (get_maxidx_smap m)  (get_bindings_smap m) ops = Some v ->
+      concrete_interpreter.ConcreteInterpreter.mload mem1 v = concrete_interpreter.ConcreteInterpreter.mload mem2 v.
+  Proof.
+    intros sstack_val_cmp ctx soffset svalue model mem strg exts m ops smem1 smem2 mem1 mem2 v.
+    intros H_sstack_val_cmp_snd H_is_sat H_is_model H_valid_soffset H_valid_svalue H_valid_smap H_valid_smem1 H_valid_smem2 H_eval_smem1 H_eval_smem2 H_eval_soffset.
+
+    unfold eval_smemory in H_eval_smem1.
+    destruct (map_option (eval_common.EvalCommon.instantiate_memory_update (fun sv : sstack_val => eval_sstack_val sv model mem strg exts (get_maxidx_smap m) (get_bindings_smap m) ops)) (U_MSTORE sstack_val soffset svalue :: smem1)) as [updates1|] eqn:E_mo_1; try discriminate.
+    injection H_eval_smem1 as H_mem1.
+
+    unfold eval_smemory in H_eval_smem2.
+    destruct (map_option (eval_common.EvalCommon.instantiate_memory_update (fun sv : sstack_val => eval_sstack_val sv model mem strg exts (get_maxidx_smap m) (get_bindings_smap m) ops)) (U_MSTORE sstack_val soffset svalue :: smem2)) as [updates2|] eqn:E_mo_2; try discriminate.
+    injection H_eval_smem2 as H_mem2.
+    
+
+    pose proof (map_option_split (memory_update sstack_val) (memory_update EVMWord) (eval_common.EvalCommon.instantiate_memory_update (fun sv : sstack_val => eval_sstack_val sv model mem strg exts (get_maxidx_smap m) (get_bindings_smap m) ops)) smem1 updates1 (U_MSTORE sstack_val soffset svalue) E_mo_1) as E_mo_1_0.
+    destruct E_mo_1_0 as [e1 [updates1' [E_updates1 [E_e1 H_mo_1_0]]]].
+
+    pose proof (map_option_split (memory_update sstack_val) (memory_update EVMWord) (eval_common.EvalCommon.instantiate_memory_update (fun sv : sstack_val => eval_sstack_val sv model mem strg exts (get_maxidx_smap m) (get_bindings_smap m) ops)) smem2 updates2 (U_MSTORE sstack_val soffset svalue) E_mo_2) as E_mo_2_0.
+    destruct E_mo_2_0 as [e2 [updates2' [E_updates2 [E_e2 H_mo_2_0]]]].
+
+
+    unfold eval_common.EvalCommon.instantiate_memory_update in E_e1.
+    unfold eval_sstack_val in E_e1.
+    rewrite H_eval_soffset in E_e1.
+    destruct (eval_sstack_val' (S (get_maxidx_smap m)) svalue model mem strg exts (get_maxidx_smap m) (get_bindings_smap m) ops) as [svalue_v|] eqn:H_eval_svalue; try discriminate.
+    injection E_e1 as E_e1.
+    
+    unfold eval_common.EvalCommon.instantiate_memory_update in E_e2.
+    unfold eval_sstack_val in E_e2.
+    rewrite H_eval_soffset in E_e2.
+    rewrite H_eval_svalue in E_e2.
+    injection E_e2 as E_e2.
+    
+    rewrite <- H_mem1.
+    rewrite <- H_mem2.
+    rewrite E_updates1.
+    rewrite E_updates2.
+    rewrite <- E_e1.
+    rewrite <- E_e2.
+
+    unfold eval_common.EvalCommon.update_memory.
+    fold eval_common.EvalCommon.update_memory.
+    unfold eval_common.EvalCommon.update_memory'.
+    
+    repeat rewrite mload_mstore_same_address.
+    reflexivity.
+  Qed.
+    
+  
+    Lemma basic_smemory_updater_remove_mstore_dups_correct:
+    forall sstack_val_cmp ctx soffset svalue model mem strg exts m ops,
+      symbolic_state_cmp.SymbolicStateCmp.safe_sstack_val_cmp_ext_1 sstack_val_cmp ->
+      is_sat ctx ->
+      is_model ctx model = true ->
+      valid_sstack_value (get_maxidx_smap m) soffset ->
+      valid_sstack_value (get_maxidx_smap m) svalue ->
+      valid_smap (get_maxidx_smap m) (get_bindings_smap m) ops ->
+      forall smem smem_r,
+      valid_smemory (get_maxidx_smap m) smem ->
+      basic_smemory_updater_remove_mstore_dups sstack_val_cmp ctx soffset smem m ops = smem_r ->
+      exists mem1 mem2,
+        eval_smemory (U_MSTORE sstack_val soffset svalue :: smem) (get_maxidx_smap m) (get_bindings_smap m) model mem strg exts ops =
+          Some mem1 /\
+          eval_smemory (U_MSTORE sstack_val soffset svalue :: smem_r) (get_maxidx_smap m) (get_bindings_smap m) model mem strg exts ops = Some mem2 /\
+          forall w, mem1 w = mem2 w.
+    Proof.
+      intros sstack_val_cmp ctx soffset svalue model mem strg exts m ops.
+      intros H_sstack_val_cmp_snd H_is_sat H_is_model H_valid_soffset H_valid_svalue H_valid_smap.
+ 
+      induction smem as [|u smem' IHsmem'].
+      + intros smem_r H_valid_smem H_basic_mstore_up.
+        simpl in H_basic_mstore_up.
+        rewrite <- H_basic_mstore_up.
+        assert(H_valid_u: valid_smemory (get_maxidx_smap m)  [U_MSTORE sstack_val soffset svalue]). simpl. auto.
+        pose proof (eval_smemory_succ (get_maxidx_smap m) (get_bindings_smap m) model mem strg exts ops [U_MSTORE sstack_val soffset svalue] H_valid_u H_valid_smap) as H_eval_u.
+        destruct H_eval_u as [smem' H_eval_u].
+        rewrite H_eval_u.
+        exists smem'.
+        exists smem'.
+        auto.
+      + intros smem_r H_valid_smem H_basic_mstore_up.
+        simpl in H_basic_mstore_up.
+        destruct u as [soffset' svalue'|soffset' svalue'] eqn:E_u.
+        (* MSTORE *)
+        ++ simpl in H_valid_smem.
+           destruct H_valid_smem as [ [H_valid_soffset' H_valid_svalue'] H_valid_smem'].
+           destruct (sstack_val_cmp (S (get_maxidx_smap m)) ctx soffset soffset' (get_maxidx_smap m) (get_bindings_smap m) (get_maxidx_smap m) (get_bindings_smap m) ops) eqn:E_cmp_soffset_soffset'.
+           +++ pose proof (IHsmem' smem_r H_valid_smem' H_basic_mstore_up) as IHsmem'_0.       
+               destruct IHsmem'_0 as [mem1' [mem2' [IHsmem'_0_1 [IHsmem'_0_2 IHsmem'_0_3]]]].
+               unfold safe_sstack_val_cmp_ext_1_d in H_sstack_val_cmp_snd.
+               unfold safe_sstack_val_cmp in H_sstack_val_cmp_snd.
+               pose proof (H_sstack_val_cmp_snd (S (get_maxidx_smap m)) (S (get_maxidx_smap m)) (Nat.le_refl (S (get_maxidx_smap m))) ctx soffset soffset' (get_maxidx_smap m) (get_bindings_smap m) (get_maxidx_smap m) (get_bindings_smap m) ops H_is_sat H_valid_soffset H_valid_soffset' H_valid_smap H_valid_smap E_cmp_soffset_soffset' model mem strg exts H_is_model) as H_eq_soffset_soffset'.
+               destruct H_eq_soffset_soffset' as [soffset_v [ H_eval_soffset H_eval_soffset']].
+
+               pose proof (two_consecutive_updates_same_address ctx soffset soffset' svalue svalue' smem' (get_maxidx_smap m) (get_bindings_smap m) model mem strg exts ops soffset_v H_is_sat H_eval_soffset H_eval_soffset' H_valid_smem' H_valid_smap H_valid_soffset H_valid_svalue H_valid_soffset' H_valid_svalue' H_is_model) as H_remove_soffset'.
+               
+               rewrite H_remove_soffset'.
+
+               rewrite IHsmem'_0_1.
+               rewrite IHsmem'_0_2.
+
+               exists mem1'.
+               exists mem2'.
+               
+               repeat split; try reflexivity.
+               apply IHsmem'_0_3.
+           +++ rewrite <- H_basic_mstore_up. 
+
+               remember (basic_smemory_updater_remove_mstore_dups sstack_val_cmp ctx soffset smem' m ops) as smem'_r.
+               rewrite Heqsmem'_r in *.
+               symmetry in Heqsmem'_r.
+               rewrite Heqsmem'_r.
+               
+               pose proof (IHsmem' smem'_r H_valid_smem' Heqsmem'_r) as IHsmem'_0.
+               destruct IHsmem'_0 as [mem1' [mem2' [H_eval_u_smem' [H_eval_u_smem'_r H_eq_mem1'_mem2']]]].
+               apply functional_extensionality in H_eq_mem1'_mem2' as H_eq_mem1'_mem2'_f.
+
+               pose proof (eval_sstack_val'_succ (S (get_maxidx_smap m)) soffset model mem strg exts (get_maxidx_smap m) (get_bindings_smap m) ops H_valid_soffset H_valid_smap (gt_Sn_n ((get_maxidx_smap m)))) as H_eval_soffset.
+               destruct H_eval_soffset as [soffset_v H_eval_soffset].
+               
+               pose proof (eval_sstack_val'_succ (S (get_maxidx_smap m)) soffset' model mem strg exts (get_maxidx_smap m) (get_bindings_smap m) ops H_valid_soffset' H_valid_smap (gt_Sn_n ((get_maxidx_smap m)))) as H_eval_soffset'.
+               destruct H_eval_soffset' as [soffset'_v H_eval_soffset'].
+
+               pose proof (eval_sstack_val'_succ (S (get_maxidx_smap m)) svalue model mem strg exts (get_maxidx_smap m) (get_bindings_smap m) ops H_valid_svalue H_valid_smap (gt_Sn_n ((get_maxidx_smap m)))) as H_eval_svalue.
+               destruct H_eval_svalue as [svlaue_v H_eval_svalue].
+
+               pose proof (eval_sstack_val'_succ (S (get_maxidx_smap m)) svalue' model mem strg exts (get_maxidx_smap m) (get_bindings_smap m) ops H_valid_svalue' H_valid_smap (gt_Sn_n ((get_maxidx_smap m)))) as H_eval_svalue'.
+               destruct H_eval_svalue' as [svlaue_v' H_eval_svalue'].
+
+               unfold eval_smemory.
+               unfold map_option.
+               repeat rewrite <- map_option_ho.
+
+               unfold eval_common.EvalCommon.instantiate_memory_update at 1.
+               unfold eval_sstack_val.
+               rewrite H_eval_soffset.
+               rewrite H_eval_svalue.
+
+               unfold eval_common.EvalCommon.instantiate_memory_update at 1.
+               unfold eval_sstack_val.
+               rewrite H_eval_soffset'.
+               rewrite H_eval_svalue'.
+              
+               unfold eval_common.EvalCommon.instantiate_memory_update at 2.
+               rewrite H_eval_soffset.
+               rewrite H_eval_svalue.
+
+               unfold eval_common.EvalCommon.instantiate_memory_update at 2.
+               unfold eval_sstack_val.
+               rewrite H_eval_soffset'.
+               rewrite H_eval_svalue'.
+
+               unfold eval_smemory in H_eval_u_smem'.
+               unfold eval_sstack_val in  H_eval_u_smem'.
+               
+
+               destruct (map_option (eval_common.EvalCommon.instantiate_memory_update (fun sv : sstack_val => eval_sstack_val'  (S (get_maxidx_smap m)) sv model mem strg exts (get_maxidx_smap m) (get_bindings_smap m) ops)) (U_MSTORE sstack_val soffset svalue :: smem')) as [updates1|] eqn:E_mo_1; try discriminate.
+               pose proof (map_option_split (memory_update sstack_val) (memory_update EVMWord) (eval_common.EvalCommon.instantiate_memory_update (fun sv : sstack_val => eval_sstack_val' (S (get_maxidx_smap m)) sv model mem strg exts (get_maxidx_smap m) (get_bindings_smap m) ops)) smem' updates1 (U_MSTORE sstack_val soffset svalue) E_mo_1) as E_mo_1_split.
+               destruct E_mo_1_split as [e1 [smem'' [E_updates_1 [E_mo_1_0 E_mo_1_1]]]].
+               rewrite E_mo_1_1.
+
+               unfold eval_smemory in H_eval_u_smem'_r.
+               unfold eval_sstack_val in  H_eval_u_smem'_r.
+               destruct (map_option (eval_common.EvalCommon.instantiate_memory_update (fun sv : sstack_val => eval_sstack_val'  (S (get_maxidx_smap m)) sv model mem strg exts (get_maxidx_smap m) (get_bindings_smap m) ops)) (U_MSTORE sstack_val soffset svalue :: smem'_r)) as [updates2|] eqn:E_mo_2; try discriminate.
+               pose proof (map_option_split (memory_update sstack_val) (memory_update EVMWord) (eval_common.EvalCommon.instantiate_memory_update (fun sv : sstack_val => eval_sstack_val' (S (get_maxidx_smap m)) sv model mem strg exts (get_maxidx_smap m) (get_bindings_smap m) ops)) smem'_r updates2 (U_MSTORE sstack_val soffset svalue) E_mo_2) as E_mo_2_split.
+               destruct E_mo_2_split as [e2 [smem'_r' [E_updates_2 [E_mo_2_0 E_mo_2_1]]]].
+               rewrite E_mo_2_1.
+
+               exists (eval_common.EvalCommon.update_memory mem (U_MSTORE EVMWord soffset_v svlaue_v :: U_MSTORE EVMWord soffset'_v svlaue_v' :: smem'')).
+               exists (eval_common.EvalCommon.update_memory mem (U_MSTORE EVMWord soffset_v svlaue_v :: U_MSTORE EVMWord soffset'_v svlaue_v' :: smem'_r')).
+	       split. reflexivity.
+               split. reflexivity.
+               intro w.
+               
+               unfold eval_common.EvalCommon.update_memory.
+               fold eval_common.EvalCommon.update_memory.
+
+               unfold eval_common.EvalCommon.instantiate_memory_update in E_mo_1_0.
+               rewrite H_eval_soffset in E_mo_1_0.
+               rewrite H_eval_svalue in E_mo_1_0.
+               injection E_mo_1_0 as E_e1.
+               
+               unfold eval_common.EvalCommon.instantiate_memory_update in E_mo_2_0.
+               rewrite H_eval_soffset in E_mo_2_0.
+               rewrite H_eval_svalue in E_mo_2_0.
+               injection E_mo_2_0 as E_e2.
+
+               rewrite E_updates_1 in H_eval_u_smem'.
+               unfold eval_common.EvalCommon.update_memory in H_eval_u_smem'.
+               fold eval_common.EvalCommon.update_memory in H_eval_u_smem'.
+               injection H_eval_u_smem' as H_eval_u_smem'.
+
+               rewrite E_updates_2 in H_eval_u_smem'_r.
+               unfold eval_common.EvalCommon.update_memory in H_eval_u_smem'_r.
+               fold eval_common.EvalCommon.update_memory in H_eval_u_smem'_r.
+               injection H_eval_u_smem'_r as H_eval_u_smem'_r.
+               rewrite H_eq_mem1'_mem2'_f in H_eval_u_smem'.
+               rewrite <- H_eval_u_smem'_r in H_eval_u_smem'.
+
+               rewrite <- E_e1 in H_eval_u_smem'.
+               rewrite <- E_e2 in H_eval_u_smem'.
+
+               apply mem_eq_after_update.
+               rewrite H_eval_u_smem'.
+               reflexivity.
+
+        (* MSTOR8 *)
+        ++ simpl in H_valid_smem.
+           destruct H_valid_smem as [ [H_valid_soffset' H_valid_svalue'] H_valid_smem'].
+           destruct (mstore8_is_included_in_mstore sstack_val_cmp ctx soffset' soffset) eqn:E_mstore8_inc.
+           +++ pose proof (IHsmem' smem_r H_valid_smem' H_basic_mstore_up) as IHsmem'_0.
+               destruct IHsmem'_0 as [mem1' [mem2' [IHsmem'_0_1 [IHsmem'_0_2 IHsmem'_0_3]]]].
+
+
+               pose proof (H_mstore8_is_included_in_mstore sstack_val_cmp ctx soffset' soffset (get_maxidx_smap m) (get_bindings_smap m) ops H_sstack_val_cmp_snd H_valid_smap H_valid_soffset' H_valid_soffset E_mstore8_inc model mem strg exts H_is_model) as E_mstore8_not_inc.
+               destruct E_mstore8_not_inc as [soffset'_v [soffset_v [H_eval_soffset' [H_eval_soffset H_addr_inc]]]].
+               
+               pose proof (two_consecutive_updates_same_address_mstore8 ctx soffset' soffset svalue' svalue smem' (get_maxidx_smap m) (get_bindings_smap m) model mem strg exts ops soffset'_v soffset_v H_is_sat H_eval_soffset' H_eval_soffset H_valid_smem' H_valid_smap H_valid_soffset' H_valid_svalue' H_valid_soffset H_valid_svalue H_is_model H_addr_inc) as H_remove_soffset'.
+
+               rewrite H_remove_soffset'.
+
+               rewrite IHsmem'_0_1.
+               rewrite IHsmem'_0_2.
+
+               exists mem1'.
+               exists mem2'.
+               
+               repeat split; try reflexivity.
+               apply IHsmem'_0_3.
+
+           +++ rewrite <- H_basic_mstore_up. 
+
+               remember (basic_smemory_updater_remove_mstore_dups sstack_val_cmp ctx soffset smem' m ops) as smem'_r.
+               rewrite Heqsmem'_r in *.
+               symmetry in Heqsmem'_r.
+               rewrite Heqsmem'_r.
+               
+               pose proof (IHsmem' smem'_r H_valid_smem' Heqsmem'_r) as IHsmem'_0.
+               destruct IHsmem'_0 as [mem1' [mem2' [H_eval_u_smem' [H_eval_u_smem'_r H_eq_mem1'_mem2']]]].
+               apply functional_extensionality in H_eq_mem1'_mem2' as H_eq_mem1'_mem2'_f.
+
+               pose proof (eval_sstack_val'_succ (S (get_maxidx_smap m)) soffset model mem strg exts (get_maxidx_smap m) (get_bindings_smap m) ops H_valid_soffset H_valid_smap (gt_Sn_n ((get_maxidx_smap m)))) as H_eval_soffset.
+               destruct H_eval_soffset as [soffset_v H_eval_soffset].
+               
+               pose proof (eval_sstack_val'_succ (S (get_maxidx_smap m)) soffset' model mem strg exts (get_maxidx_smap m) (get_bindings_smap m) ops H_valid_soffset' H_valid_smap (gt_Sn_n ((get_maxidx_smap m)))) as H_eval_soffset'.
+               destruct H_eval_soffset' as [soffset'_v H_eval_soffset'].
+
+               pose proof (eval_sstack_val'_succ (S (get_maxidx_smap m)) svalue model mem strg exts (get_maxidx_smap m) (get_bindings_smap m) ops H_valid_svalue H_valid_smap (gt_Sn_n ((get_maxidx_smap m)))) as H_eval_svalue.
+               destruct H_eval_svalue as [svlaue_v H_eval_svalue].
+
+               pose proof (eval_sstack_val'_succ (S (get_maxidx_smap m)) svalue' model mem strg exts (get_maxidx_smap m) (get_bindings_smap m) ops H_valid_svalue' H_valid_smap (gt_Sn_n ((get_maxidx_smap m)))) as H_eval_svalue'.
+               destruct H_eval_svalue' as [svlaue_v' H_eval_svalue'].
+
+               unfold eval_smemory.
+               unfold map_option.
+               repeat rewrite <- map_option_ho.
+
+               unfold eval_common.EvalCommon.instantiate_memory_update at 1.
+               unfold eval_sstack_val.
+               rewrite H_eval_soffset.
+               rewrite H_eval_svalue.
+
+               unfold eval_common.EvalCommon.instantiate_memory_update at 1.
+               unfold eval_sstack_val.
+               rewrite H_eval_soffset'.
+               rewrite H_eval_svalue'.
+              
+               unfold eval_common.EvalCommon.instantiate_memory_update at 2.
+               rewrite H_eval_soffset.
+               rewrite H_eval_svalue.
+
+               unfold eval_common.EvalCommon.instantiate_memory_update at 2.
+               unfold eval_sstack_val.
+               rewrite H_eval_soffset'.
+               rewrite H_eval_svalue'.
+
+               unfold eval_smemory in H_eval_u_smem'.
+               unfold eval_sstack_val in  H_eval_u_smem'.
+               
+
+               destruct (map_option (eval_common.EvalCommon.instantiate_memory_update (fun sv : sstack_val => eval_sstack_val'  (S (get_maxidx_smap m)) sv model mem strg exts (get_maxidx_smap m) (get_bindings_smap m) ops)) (U_MSTORE sstack_val soffset svalue :: smem')) as [updates1|] eqn:E_mo_1; try discriminate.
+               pose proof (map_option_split (memory_update sstack_val) (memory_update EVMWord) (eval_common.EvalCommon.instantiate_memory_update (fun sv : sstack_val => eval_sstack_val' (S (get_maxidx_smap m)) sv model mem strg exts (get_maxidx_smap m) (get_bindings_smap m) ops)) smem' updates1 (U_MSTORE sstack_val soffset svalue) E_mo_1) as E_mo_1_split.
+               destruct E_mo_1_split as [e1 [smem'' [E_updates_1 [E_mo_1_0 E_mo_1_1]]]].
+               rewrite E_mo_1_1.
+
+               unfold eval_smemory in H_eval_u_smem'_r.
+               unfold eval_sstack_val in  H_eval_u_smem'_r.
+               destruct (map_option (eval_common.EvalCommon.instantiate_memory_update (fun sv : sstack_val => eval_sstack_val'  (S (get_maxidx_smap m)) sv model mem strg exts (get_maxidx_smap m) (get_bindings_smap m) ops)) (U_MSTORE sstack_val soffset svalue :: smem'_r)) as [updates2|] eqn:E_mo_2; try discriminate.
+               pose proof (map_option_split (memory_update sstack_val) (memory_update EVMWord) (eval_common.EvalCommon.instantiate_memory_update (fun sv : sstack_val => eval_sstack_val' (S (get_maxidx_smap m)) sv model mem strg exts (get_maxidx_smap m) (get_bindings_smap m) ops)) smem'_r updates2 (U_MSTORE sstack_val soffset svalue) E_mo_2) as E_mo_2_split.
+               destruct E_mo_2_split as [e2 [smem'_r' [E_updates_2 [E_mo_2_0 E_mo_2_1]]]].
+               rewrite E_mo_2_1.
+
+               exists (eval_common.EvalCommon.update_memory mem (U_MSTORE EVMWord soffset_v svlaue_v :: U_MSTORE8 EVMWord soffset'_v svlaue_v' :: smem'')).
+               exists (eval_common.EvalCommon.update_memory mem (U_MSTORE EVMWord soffset_v svlaue_v :: U_MSTORE8 EVMWord soffset'_v svlaue_v' :: smem'_r')).
+	       split. reflexivity.
+               split. reflexivity.
+               intro w.
+               
+               unfold eval_common.EvalCommon.update_memory.
+               fold eval_common.EvalCommon.update_memory.
+
+               unfold eval_common.EvalCommon.instantiate_memory_update in E_mo_1_0.
+               rewrite H_eval_soffset in E_mo_1_0.
+               rewrite H_eval_svalue in E_mo_1_0.
+               injection E_mo_1_0 as E_e1.
+               
+               unfold eval_common.EvalCommon.instantiate_memory_update in E_mo_2_0.
+               rewrite H_eval_soffset in E_mo_2_0.
+               rewrite H_eval_svalue in E_mo_2_0.
+               injection E_mo_2_0 as E_e2.
+
+               rewrite E_updates_1 in H_eval_u_smem'.
+               unfold eval_common.EvalCommon.update_memory in H_eval_u_smem'.
+               fold eval_common.EvalCommon.update_memory in H_eval_u_smem'.
+               injection H_eval_u_smem' as H_eval_u_smem'.
+
+               rewrite E_updates_2 in H_eval_u_smem'_r.
+               unfold eval_common.EvalCommon.update_memory in H_eval_u_smem'_r.
+               fold eval_common.EvalCommon.update_memory in H_eval_u_smem'_r.
+               injection H_eval_u_smem'_r as H_eval_u_smem'_r.
+               rewrite H_eq_mem1'_mem2'_f in H_eval_u_smem'.
+               rewrite <- H_eval_u_smem'_r in H_eval_u_smem'.
+
+               rewrite <- E_e1 in H_eval_u_smem'.
+               rewrite <- E_e2 in H_eval_u_smem'.
+
+               apply mem_eq_after_update.
+               rewrite H_eval_u_smem'.
+               reflexivity.
+Qed.
+
+
+
+    Lemma basic_smemory_updater_remove_mstore8_dups_correct:
+      forall sstack_val_cmp ctx soffset svalue model mem strg exts m ops,
+        symbolic_state_cmp.SymbolicStateCmp.safe_sstack_val_cmp_ext_1 sstack_val_cmp ->
+        is_sat ctx ->
+        is_model ctx model = true ->
+        valid_sstack_value (get_maxidx_smap m) soffset ->
+        valid_sstack_value (get_maxidx_smap m) svalue ->
+        valid_smap (get_maxidx_smap m) (get_bindings_smap m) ops ->
+        forall smem smem',
+          valid_smemory (get_maxidx_smap m) smem ->
+          basic_smemory_updater_remove_mstore8_dups sstack_val_cmp ctx soffset smem m ops = smem' ->
+          exists mem1 mem2,
+            eval_smemory (U_MSTORE8 sstack_val soffset svalue :: smem) (get_maxidx_smap m) (get_bindings_smap m) model mem strg exts ops =
+          Some mem1 /\
+              eval_smemory (U_MSTORE8 sstack_val soffset svalue :: smem') (get_maxidx_smap m) (get_bindings_smap m) model mem strg exts ops = Some mem2 /\
+              forall w, mem1 w = mem2 w.
+    Proof.
+      intros sstack_val_cmp ctx soffset svalue model mem strg exts m ops.
+      intros H_sstack_val_cmp_snd H_is_sat H_is_model H_valid_soffset H_valid_svalue H_valid_smap.
+ 
+      induction smem as [|u smem' IHsmem'].
+      + intros smem_r H_valid_smem H_basic_mstore_up.
+        simpl in H_basic_mstore_up.
+        rewrite <- H_basic_mstore_up.
+        assert(H_valid_u: valid_smemory (get_maxidx_smap m)  [U_MSTORE sstack_val soffset svalue]). simpl. auto.
+        pose proof (eval_smemory_succ (get_maxidx_smap m) (get_bindings_smap m) model mem strg exts ops [U_MSTORE8 sstack_val soffset svalue] H_valid_u H_valid_smap) as H_eval_u.
+        destruct H_eval_u as [smem' H_eval_u].
+        rewrite H_eval_u.
+        exists smem'.
+        exists smem'.
+        auto.
+      + intros smem_r H_valid_smem H_basic_mstore_up.
+        simpl in H_basic_mstore_up.
+        destruct u as [soffset' svalue'|soffset' svalue'] eqn:E_u.
+        (* MSTORE *)
+        ++ simpl in H_valid_smem.
+           destruct H_valid_smem as [ [H_valid_soffset' H_valid_svalue'] H_valid_smem'].
+
+           rewrite <- H_basic_mstore_up. 
+
+           remember (basic_smemory_updater_remove_mstore8_dups sstack_val_cmp ctx soffset smem' m ops) as smem'_r.
+           rewrite Heqsmem'_r in *.
+           symmetry in Heqsmem'_r.
+           rewrite Heqsmem'_r.
+               
+           pose proof (IHsmem' smem'_r H_valid_smem' Heqsmem'_r) as IHsmem'_0.
+           destruct IHsmem'_0 as [mem1' [mem2' [H_eval_u_smem' [H_eval_u_smem'_r H_eq_mem1'_mem2']]]].
+           apply functional_extensionality in H_eq_mem1'_mem2' as H_eq_mem1'_mem2'_f.
+           
+           pose proof (eval_sstack_val'_succ (S (get_maxidx_smap m)) soffset model mem strg exts (get_maxidx_smap m) (get_bindings_smap m) ops H_valid_soffset H_valid_smap (gt_Sn_n ((get_maxidx_smap m)))) as H_eval_soffset.
+           destruct H_eval_soffset as [soffset_v H_eval_soffset].
+           
+           pose proof (eval_sstack_val'_succ (S (get_maxidx_smap m)) soffset' model mem strg exts (get_maxidx_smap m) (get_bindings_smap m) ops H_valid_soffset' H_valid_smap (gt_Sn_n ((get_maxidx_smap m)))) as H_eval_soffset'.
+           destruct H_eval_soffset' as [soffset'_v H_eval_soffset'].
+           
+           pose proof (eval_sstack_val'_succ (S (get_maxidx_smap m)) svalue model mem strg exts (get_maxidx_smap m) (get_bindings_smap m) ops H_valid_svalue H_valid_smap (gt_Sn_n ((get_maxidx_smap m)))) as H_eval_svalue.
+           destruct H_eval_svalue as [svlaue_v H_eval_svalue].
+           
+           pose proof (eval_sstack_val'_succ (S (get_maxidx_smap m)) svalue' model mem strg exts (get_maxidx_smap m) (get_bindings_smap m) ops H_valid_svalue' H_valid_smap (gt_Sn_n ((get_maxidx_smap m)))) as H_eval_svalue'.
+           destruct H_eval_svalue' as [svlaue_v' H_eval_svalue'].
+           
+           unfold eval_smemory.
+           unfold map_option.
+           repeat rewrite <- map_option_ho.
+           
+           unfold eval_common.EvalCommon.instantiate_memory_update at 1.
+           unfold eval_sstack_val.
+           rewrite H_eval_soffset.
+           rewrite H_eval_svalue.
+           
+           unfold eval_common.EvalCommon.instantiate_memory_update at 1.
+           unfold eval_sstack_val.
+           rewrite H_eval_soffset'.
+           rewrite H_eval_svalue'.
+           
+           unfold eval_common.EvalCommon.instantiate_memory_update at 2.
+           rewrite H_eval_soffset.
+           rewrite H_eval_svalue.
+           
+           unfold eval_common.EvalCommon.instantiate_memory_update at 2.
+           unfold eval_sstack_val.
+           rewrite H_eval_soffset'.
+           rewrite H_eval_svalue'.
+           
+           unfold eval_smemory in H_eval_u_smem'.
+           unfold eval_sstack_val in  H_eval_u_smem'.
+           
+
+           destruct (map_option (eval_common.EvalCommon.instantiate_memory_update (fun sv : sstack_val => eval_sstack_val'  (S (get_maxidx_smap m)) sv model mem strg exts (get_maxidx_smap m) (get_bindings_smap m) ops)) (U_MSTORE8 sstack_val soffset svalue :: smem')) as [updates1|] eqn:E_mo_1; try discriminate.
+           pose proof (map_option_split (memory_update sstack_val) (memory_update EVMWord) (eval_common.EvalCommon.instantiate_memory_update (fun sv : sstack_val => eval_sstack_val' (S (get_maxidx_smap m)) sv model mem strg exts (get_maxidx_smap m) (get_bindings_smap m) ops)) smem' updates1 (U_MSTORE8 sstack_val soffset svalue) E_mo_1) as E_mo_1_split.
+           destruct E_mo_1_split as [e1 [smem'' [E_updates_1 [E_mo_1_0 E_mo_1_1]]]].
+           rewrite E_mo_1_1.
+
+           unfold eval_smemory in H_eval_u_smem'_r.
+           unfold eval_sstack_val in  H_eval_u_smem'_r.
+           destruct (map_option (eval_common.EvalCommon.instantiate_memory_update (fun sv : sstack_val => eval_sstack_val'  (S (get_maxidx_smap m)) sv model mem strg exts (get_maxidx_smap m) (get_bindings_smap m) ops)) (U_MSTORE8 sstack_val soffset svalue :: smem'_r)) as [updates2|] eqn:E_mo_2; try discriminate.
+           pose proof (map_option_split (memory_update sstack_val) (memory_update EVMWord) (eval_common.EvalCommon.instantiate_memory_update (fun sv : sstack_val => eval_sstack_val' (S (get_maxidx_smap m)) sv model mem strg exts (get_maxidx_smap m) (get_bindings_smap m) ops)) smem'_r updates2 (U_MSTORE8 sstack_val soffset svalue) E_mo_2) as E_mo_2_split.
+           destruct E_mo_2_split as [e2 [smem'_r' [E_updates_2 [E_mo_2_0 E_mo_2_1]]]].
+           rewrite E_mo_2_1.
+           
+           exists (eval_common.EvalCommon.update_memory mem (U_MSTORE8 EVMWord soffset_v svlaue_v :: U_MSTORE EVMWord soffset'_v svlaue_v' :: smem'')).
+           exists (eval_common.EvalCommon.update_memory mem (U_MSTORE8 EVMWord soffset_v svlaue_v :: U_MSTORE EVMWord soffset'_v svlaue_v' :: smem'_r')).
+	   split. reflexivity.
+           split. reflexivity.
+           intro w.
+           
+           unfold eval_common.EvalCommon.update_memory.
+           fold eval_common.EvalCommon.update_memory.
+           
+           unfold eval_common.EvalCommon.instantiate_memory_update in E_mo_1_0.
+           rewrite H_eval_soffset in E_mo_1_0.
+           rewrite H_eval_svalue in E_mo_1_0.
+           injection E_mo_1_0 as E_e1.
+           
+           unfold eval_common.EvalCommon.instantiate_memory_update in E_mo_2_0.
+           rewrite H_eval_soffset in E_mo_2_0.
+           rewrite H_eval_svalue in E_mo_2_0.
+           injection E_mo_2_0 as E_e2.
+           
+           rewrite E_updates_1 in H_eval_u_smem'.
+           unfold eval_common.EvalCommon.update_memory in H_eval_u_smem'.
+           fold eval_common.EvalCommon.update_memory in H_eval_u_smem'.
+           injection H_eval_u_smem' as H_eval_u_smem'.
+           
+           rewrite E_updates_2 in H_eval_u_smem'_r.
+           unfold eval_common.EvalCommon.update_memory in H_eval_u_smem'_r.
+           fold eval_common.EvalCommon.update_memory in H_eval_u_smem'_r.
+           injection H_eval_u_smem'_r as H_eval_u_smem'_r.
+           rewrite H_eq_mem1'_mem2'_f in H_eval_u_smem'.
+           rewrite <- H_eval_u_smem'_r in H_eval_u_smem'.
+           
+           rewrite <- E_e1 in H_eval_u_smem'.
+           rewrite <- E_e2 in H_eval_u_smem'.
+
+           apply mem_eq_after_update.
+           rewrite H_eval_u_smem'.
+           reflexivity.
+
+
+        (* MSTORE8 *)
+        ++ simpl in H_valid_smem.
+           destruct H_valid_smem as [ [H_valid_soffset' H_valid_svalue'] H_valid_smem'].
+           destruct (sstack_val_cmp (S (get_maxidx_smap m)) ctx soffset soffset' (get_maxidx_smap m) (get_bindings_smap m) (get_maxidx_smap m) (get_bindings_smap m) ops) eqn:E_cmp_soffset_soffset'.
+           +++ pose proof (IHsmem' smem_r H_valid_smem' H_basic_mstore_up) as IHsmem'_0.       
+               destruct IHsmem'_0 as [mem1' [mem2' [IHsmem'_0_1 [IHsmem'_0_2 IHsmem'_0_3]]]].
+               unfold safe_sstack_val_cmp_ext_1_d in H_sstack_val_cmp_snd.
+               unfold safe_sstack_val_cmp in H_sstack_val_cmp_snd.
+               pose proof (H_sstack_val_cmp_snd (S (get_maxidx_smap m)) (S (get_maxidx_smap m)) (Nat.le_refl (S (get_maxidx_smap m))) ctx soffset soffset' (get_maxidx_smap m) (get_bindings_smap m) (get_maxidx_smap m) (get_bindings_smap m) ops H_is_sat H_valid_soffset H_valid_soffset' H_valid_smap H_valid_smap E_cmp_soffset_soffset' model mem strg exts H_is_model) as H_eq_soffset_soffset'.
+               destruct H_eq_soffset_soffset' as [soffset_v [ H_eval_soffset H_eval_soffset']].
+
+               pose proof (two_consecutive_mstore8_updates_same_address ctx soffset soffset' svalue svalue' smem' (get_maxidx_smap m) (get_bindings_smap m) model mem strg exts ops soffset_v H_is_sat H_eval_soffset H_eval_soffset' H_valid_smem' H_valid_smap H_valid_soffset H_valid_svalue H_valid_soffset' H_valid_svalue' H_is_model) as H_remove_soffset'.
+               rewrite H_remove_soffset'.
+
+               rewrite IHsmem'_0_1.
+               rewrite IHsmem'_0_2.
+
+               exists mem1'.
+               exists mem2'.
+               
+               repeat split; try reflexivity.
+               apply IHsmem'_0_3.
+           +++ rewrite <- H_basic_mstore_up. 
+
+               remember (basic_smemory_updater_remove_mstore8_dups sstack_val_cmp ctx soffset smem' m ops) as smem'_r.
+               rewrite Heqsmem'_r in *.
+               symmetry in Heqsmem'_r.
+               rewrite Heqsmem'_r.
+               
+               pose proof (IHsmem' smem'_r H_valid_smem' Heqsmem'_r) as IHsmem'_0.
+               destruct IHsmem'_0 as [mem1' [mem2' [H_eval_u_smem' [H_eval_u_smem'_r H_eq_mem1'_mem2']]]].
+               apply functional_extensionality in H_eq_mem1'_mem2' as H_eq_mem1'_mem2'_f.
+
+               pose proof (eval_sstack_val'_succ (S (get_maxidx_smap m)) soffset model mem strg exts (get_maxidx_smap m) (get_bindings_smap m) ops H_valid_soffset H_valid_smap (gt_Sn_n ((get_maxidx_smap m)))) as H_eval_soffset.
+               destruct H_eval_soffset as [soffset_v H_eval_soffset].
+               
+               pose proof (eval_sstack_val'_succ (S (get_maxidx_smap m)) soffset' model mem strg exts (get_maxidx_smap m) (get_bindings_smap m) ops H_valid_soffset' H_valid_smap (gt_Sn_n ((get_maxidx_smap m)))) as H_eval_soffset'.
+               destruct H_eval_soffset' as [soffset'_v H_eval_soffset'].
+
+               pose proof (eval_sstack_val'_succ (S (get_maxidx_smap m)) svalue model mem strg exts (get_maxidx_smap m) (get_bindings_smap m) ops H_valid_svalue H_valid_smap (gt_Sn_n ((get_maxidx_smap m)))) as H_eval_svalue.
+               destruct H_eval_svalue as [svlaue_v H_eval_svalue].
+
+               pose proof (eval_sstack_val'_succ (S (get_maxidx_smap m)) svalue' model mem strg exts (get_maxidx_smap m) (get_bindings_smap m) ops H_valid_svalue' H_valid_smap (gt_Sn_n ((get_maxidx_smap m)))) as H_eval_svalue'.
+               destruct H_eval_svalue' as [svlaue_v' H_eval_svalue'].
+
+               unfold eval_smemory.
+               unfold map_option.
+               repeat rewrite <- map_option_ho.
+
+               unfold eval_common.EvalCommon.instantiate_memory_update at 1.
+               unfold eval_sstack_val.
+               rewrite H_eval_soffset.
+               rewrite H_eval_svalue.
+
+               unfold eval_common.EvalCommon.instantiate_memory_update at 1.
+               unfold eval_sstack_val.
+               rewrite H_eval_soffset'.
+               rewrite H_eval_svalue'.
+              
+               unfold eval_common.EvalCommon.instantiate_memory_update at 2.
+               rewrite H_eval_soffset.
+               rewrite H_eval_svalue.
+
+               unfold eval_common.EvalCommon.instantiate_memory_update at 2.
+               unfold eval_sstack_val.
+               rewrite H_eval_soffset'.
+               rewrite H_eval_svalue'.
+
+               unfold eval_smemory in H_eval_u_smem'.
+               unfold eval_sstack_val in  H_eval_u_smem'.
+               
+
+               destruct (map_option (eval_common.EvalCommon.instantiate_memory_update (fun sv : sstack_val => eval_sstack_val'  (S (get_maxidx_smap m)) sv model mem strg exts (get_maxidx_smap m) (get_bindings_smap m) ops)) (U_MSTORE8 sstack_val soffset svalue :: smem')) as [updates1|] eqn:E_mo_1; try discriminate.
+               pose proof (map_option_split (memory_update sstack_val) (memory_update EVMWord) (eval_common.EvalCommon.instantiate_memory_update (fun sv : sstack_val => eval_sstack_val' (S (get_maxidx_smap m)) sv model mem strg exts (get_maxidx_smap m) (get_bindings_smap m) ops)) smem' updates1 (U_MSTORE8 sstack_val soffset svalue) E_mo_1) as E_mo_1_split.
+               destruct E_mo_1_split as [e1 [smem'' [E_updates_1 [E_mo_1_0 E_mo_1_1]]]].
+               rewrite E_mo_1_1.
+
+               unfold eval_smemory in H_eval_u_smem'_r.
+               unfold eval_sstack_val in  H_eval_u_smem'_r.
+               destruct (map_option (eval_common.EvalCommon.instantiate_memory_update (fun sv : sstack_val => eval_sstack_val'  (S (get_maxidx_smap m)) sv model mem strg exts (get_maxidx_smap m) (get_bindings_smap m) ops)) (U_MSTORE8 sstack_val soffset svalue :: smem'_r)) as [updates2|] eqn:E_mo_2; try discriminate.
+               pose proof (map_option_split (memory_update sstack_val) (memory_update EVMWord) (eval_common.EvalCommon.instantiate_memory_update (fun sv : sstack_val => eval_sstack_val' (S (get_maxidx_smap m)) sv model mem strg exts (get_maxidx_smap m) (get_bindings_smap m) ops)) smem'_r updates2 (U_MSTORE8 sstack_val soffset svalue) E_mo_2) as E_mo_2_split.
+               destruct E_mo_2_split as [e2 [smem'_r' [E_updates_2 [E_mo_2_0 E_mo_2_1]]]].
+               rewrite E_mo_2_1.
+
+               exists (eval_common.EvalCommon.update_memory mem (U_MSTORE8 EVMWord soffset_v svlaue_v :: U_MSTORE8 EVMWord soffset'_v svlaue_v' :: smem'')).
+               exists (eval_common.EvalCommon.update_memory mem (U_MSTORE8 EVMWord soffset_v svlaue_v :: U_MSTORE8 EVMWord soffset'_v svlaue_v' :: smem'_r')).
+	       split. reflexivity.
+               split. reflexivity.
+               intro w.
+               
+               unfold eval_common.EvalCommon.update_memory.
+               fold eval_common.EvalCommon.update_memory.
+
+               unfold eval_common.EvalCommon.instantiate_memory_update in E_mo_1_0.
+               rewrite H_eval_soffset in E_mo_1_0.
+               rewrite H_eval_svalue in E_mo_1_0.
+               injection E_mo_1_0 as E_e1.
+               
+               unfold eval_common.EvalCommon.instantiate_memory_update in E_mo_2_0.
+               rewrite H_eval_soffset in E_mo_2_0.
+               rewrite H_eval_svalue in E_mo_2_0.
+               injection E_mo_2_0 as E_e2.
+
+               rewrite E_updates_1 in H_eval_u_smem'.
+               unfold eval_common.EvalCommon.update_memory in H_eval_u_smem'.
+               fold eval_common.EvalCommon.update_memory in H_eval_u_smem'.
+               injection H_eval_u_smem' as H_eval_u_smem'.
+
+               rewrite E_updates_2 in H_eval_u_smem'_r.
+               unfold eval_common.EvalCommon.update_memory in H_eval_u_smem'_r.
+               fold eval_common.EvalCommon.update_memory in H_eval_u_smem'_r.
+               injection H_eval_u_smem'_r as H_eval_u_smem'_r.
+               rewrite H_eq_mem1'_mem2'_f in H_eval_u_smem'.
+               rewrite <- H_eval_u_smem'_r in H_eval_u_smem'.
+
+               rewrite <- E_e1 in H_eval_u_smem'.
+               rewrite <- E_e2 in H_eval_u_smem'.
+
+               apply mem_eq_after_update.
+               rewrite H_eval_u_smem'.
+               reflexivity.
+    Qed.
+      
+
+
+  Lemma basic_smemory_updater_snd: smemory_updater_ext_snd basic_smemory_updater.
+    unfold smemory_updater_ext_snd.
+    intros sstack_val_cmp H_sstack_val_cmp_snd.
+    unfold smemory_updater_snd.
+    split.
+      (* Validity *)
+    + apply basic_smemory_updater_valid.
+      apply H_sstack_val_cmp_snd. 
+    + unfold smemory_updater_correct_res.
+      intros ctx m smem smem' u ops H_is_sat H_valid_smap H_valid_smem H_valid_u H_basic_smem_updater.
+      intros model mem strg exts H_is_model.
+      unfold basic_smemory_updater in H_basic_smem_updater.
+      destruct u as [soffset svalue|soffset svalue] eqn:E_u.
+      ++ simpl in H_valid_u.
+         destruct H_valid_u as [H_valid_soffset H_valid_svalue].
+         destruct smem' as [|u' smem'']; try discriminate.
+         injection H_basic_smem_updater as H_u' H_smem''.
+         pose proof (basic_smemory_updater_remove_mstore_dups_correct sstack_val_cmp ctx soffset svalue model mem strg exts m ops H_sstack_val_cmp_snd H_is_sat H_is_model H_valid_soffset H_valid_svalue H_valid_smap smem smem''  H_valid_smem H_smem'') as H_basic_smemory_updater_remove_mstore_dups_correct.
+         destruct H_basic_smemory_updater_remove_mstore_dups_correct as [mem1 [mem2 H_basic_smemory_updater_remove_mstore_dups_correct]].
+         destruct H_basic_smemory_updater_remove_mstore_dups_correct as [H_mem1 [H_mem2 H_eq_mem1_mem2]].
+         rewrite <- H_u'.
+         rewrite H_mem1.
+         rewrite H_mem2.
+         exists mem1.
+         exists mem2.
+         repeat split; try reflexivity.
+         unfold eq_memory.
+         apply H_eq_mem1_mem2.
+      ++ simpl in H_valid_u.
+         destruct H_valid_u as [H_valid_soffset H_valid_svalue].
+         destruct smem' as [|u' smem'']; try discriminate.
+         injection H_basic_smem_updater as H_u' H_smem''.
+         pose proof (basic_smemory_updater_remove_mstore8_dups_correct sstack_val_cmp ctx soffset svalue model mem strg exts m ops H_sstack_val_cmp_snd H_is_sat H_is_model H_valid_soffset H_valid_svalue H_valid_smap smem smem''  H_valid_smem H_smem'') as H_basic_smemory_updater_remove_mstore8_dups_correct.
+         destruct H_basic_smemory_updater_remove_mstore8_dups_correct as [mem1 [mem2 H_basic_smemory_updater_remove_mstore8_dups_correct]].
+         destruct H_basic_smemory_updater_remove_mstore8_dups_correct as [H_mem1 [H_mem2 H_eq_mem1_mem2]].
+         rewrite <- H_u'.
+         rewrite H_mem1.
+         rewrite H_mem2.
+         exists mem1.
+         exists mem2.
+         repeat split; try reflexivity.
+         unfold eq_memory.
+         apply H_eq_mem1_mem2.
+  Qed.
+
+  
+
+End MemoryOpsSolversImplSoundness.
