storage_cmp_impl_soundness.v
@@ -1,0 +1,653 @@
+Require Import Arith.
+Require Import Nat.
+Require Import Bool.
+Require Import bbv.Word.
+Require Import Coq.NArith.NArith.
+Require Import List.
+Import ListNotations.
+
+Require Import Coq.Logic.FunctionalExtensionality.
+
+Require Import FORVES2.constants.
+Import Constants.
+
+Require Import FORVES2.program.
+Import Program.
+
+Require Import FORVES2.execution_state.
+Import ExecutionState.
+
+Require Import FORVES2.stack_operation_instructions.
+Import StackOpInstrs.
+
+Require Import FORVES2.misc.
+Import Misc.
+
+Require Import FORVES2.symbolic_state.
+Import SymbolicState.
+
+Require Import FORVES2.symbolic_state_eval.
+Import SymbolicStateEval.
+
+Require Import FORVES2.symbolic_state_eval_facts.
+Import SymbolicStateEvalFacts.
+
+Require Import FORVES2.valid_symbolic_state.
+Import ValidSymbolicState.
+
+Require Import FORVES2.valid_symbolic_state.
+Import ValidSymbolicState.
+
+Require Import FORVES2.symbolic_state_cmp.
+Import SymbolicStateCmp.
+
+Require Import FORVES2.storage_cmp_impl.
+Import StorageCmpImpl.
+
+Require Import FORVES2.eval_common.
+Import EvalCommon.
+
+Require Import FORVES2.constraints.
+Import Constraints.
+
+
+Module StorageCmpImplSoundness.
+
+  Theorem trivial_storage_cmp_snd:
+    safe_sstorage_cmp_ext_wrt_sstack_value_cmp trivial_storage_cmp.
+  Proof.
+    unfold safe_sstorage_cmp_ext_wrt_sstack_value_cmp.
+    unfold safe_sstack_val_cmp_ext_1_d.
+    unfold safe_sstorage_cmp_ext_d.
+    unfold safe_sstorage_cmp.
+    unfold trivial_storage_cmp.
+    intros.
+    destruct sstrg1; destruct sstrg2; try discriminate.
+    exists strg.
+    auto.
+  Qed.
+  
+
+  Theorem basic_storage_cmp_snd:
+    safe_sstorage_cmp_ext_wrt_sstack_value_cmp basic_storage_cmp.
+  Proof.
+    unfold safe_sstorage_cmp_ext_wrt_sstack_value_cmp.
+    intros d sstack_val_cmp H_sstack_val_cmp_snd.
+    unfold safe_sstorage_cmp_ext_d.
+    intros d' H_d'_le_d.
+    unfold safe_sstorage_cmp.
+    intros ctx sstrg1 sstrg2 maxidx1 sb1 maxidx2 sb2 ops H_is_sat H_valid_sb1 H_valid_sb2.
+    revert sstrg2.
+    revert sstrg1.
+    induction sstrg1 as [|u1 sstrg1' IHsstrg1'].
+    + intros sstrg2 H_valid_sstrg1 H_valid_sstrg2 H_basic_strg_smp model mem strg exts H_is_model.
+      destruct sstrg2; try discriminate.
+      exists strg.
+      unfold eval_sstorage.
+      simpl.
+      split; reflexivity.
+    + intros sstrg2 H_valid_sstrg1 H_valid_sstrg2 H_basic_strg_smp model mem strg exts H_is_model.
+      destruct sstrg2 as [|u2 sstrg2'] eqn:H_sstrg2.
+      ++ simpl in H_basic_strg_smp.
+         destruct u1.
+         discriminate.
+      ++ simpl in H_basic_strg_smp.
+         destruct u1 as [skey1 svalue1] eqn:E_u1.
+         destruct u2 as [skey2 svalue2] eqn:E_u2.
+         destruct (sstack_val_cmp d' ctx skey1 skey2 maxidx1 sb1 maxidx2 sb2 ops) eqn:E_cmp_skey1_skey2; try discriminate.
+         destruct (sstack_val_cmp d' ctx svalue1 svalue2 maxidx1 sb1 maxidx2 sb2 ops) eqn:E_cmp_svalue1_svalue2; try discriminate.
+         simpl in H_valid_sstrg1.
+         destruct H_valid_sstrg1 as [ [H_valid_skey1 H_valid_svalue1] H_valid_sstrg1'].
+         simpl in H_valid_sstrg2.
+         destruct H_valid_sstrg2 as [ [H_valid_skey2 H_valid_svalue2] H_valid_sstrg2'].
+         pose proof (IHsstrg1' sstrg2' H_valid_sstrg1' H_valid_sstrg2' H_basic_strg_smp model mem strg exts H_is_model) as IHsstrg1'_0.
+         destruct IHsstrg1'_0 as [strg' [IHsstrg1'_0 IHsstrg1'_1]].
+
+         unfold safe_sstack_val_cmp_ext_1_d in H_sstack_val_cmp_snd.
+         pose proof (H_sstack_val_cmp_snd d' H_d'_le_d) as H_sstack_val_cmp_snd_d'.
+         unfold safe_sstack_val_cmp in H_sstack_val_cmp_snd_d'.
+         pose proof(H_sstack_val_cmp_snd_d' ctx skey1 skey2 maxidx1 sb1 maxidx2 sb2 ops H_is_sat H_valid_skey1 H_valid_skey2 H_valid_sb1 H_valid_sb2 E_cmp_skey1_skey2 model mem strg exts H_is_model) as H_eval_skey1_skey2.
+         destruct H_eval_skey1_skey2 as [skey_1_2_v [H_eval_skey1 H_eval_skey2]].
+
+         pose proof(H_sstack_val_cmp_snd_d' ctx svalue1 svalue2 maxidx1 sb1 maxidx2 sb2 ops H_is_sat H_valid_svalue1 H_valid_svalue2 H_valid_sb1 H_valid_sb2 E_cmp_svalue1_svalue2 model mem strg exts H_is_model) as H_eval_svalue1_svalue2.
+         destruct H_eval_svalue1_svalue2 as [svalue_1_2_v [H_eval_svalue1 H_eval_svalue2]].
+         exists (fun key => if (key =? wordToN skey_1_2_v)%N then svalue_1_2_v else strg' key).
+
+         unfold eval_sstorage in IHsstrg1'_0.
+         destruct (map_option (instantiate_storage_update (fun sv : sstack_val => eval_sstack_val sv model mem strg exts maxidx1 sb1 ops)) sstrg1') as [updates1|] eqn:H_mo_sstrg1'; try discriminate.
+         injection IHsstrg1'_0 as IHsstrg1'_0.
+         
+         unfold eval_sstorage in IHsstrg1'_1.
+         destruct (map_option (instantiate_storage_update (fun sv : sstack_val => eval_sstack_val sv model mem strg exts maxidx2 sb2 ops)) sstrg2') as [updates2|] eqn:H_mo_sstrg2'; try discriminate.
+         injection IHsstrg1'_1 as IHsstrg1'_1.
+
+         unfold eval_sstorage.
+         unfold map_option.
+         repeat rewrite <- map_option_ho.
+
+         unfold instantiate_storage_update at 1.
+         rewrite H_eval_skey1.
+         rewrite H_eval_svalue1.
+         
+         unfold instantiate_storage_update at 2.
+         rewrite H_eval_skey2.
+         rewrite H_eval_svalue2.
+
+         rewrite H_mo_sstrg1'.
+         rewrite H_mo_sstrg2'.
+
+         unfold update_storage.
+         fold update_storage.
+
+         rewrite IHsstrg1'_0.
+         rewrite IHsstrg1'_1.
+
+         split; try reflexivity.
+  Qed.
+
+  Lemma f_v1_v2_neq:
+    forall (g : N -> EVMWord) (v1 v2:N) (w1 w2 : EVMWord),
+      (v1 =? v2)%N = false ->
+      forall x,
+      ( (fun key : N => if (key =? v1)%N then w1 else if (key =? v2)%N then w2 else g key) x)
+      =
+        ( (fun key : N => if (key =? v2)%N then w2 else if (key =? v1)%N then w1 else g key) x).
+  Proof.
+    intros g v1 v2 w1 w2 H_v1_neq_v2 x.
+    simpl.
+    destruct (x =? v1)%N eqn:E_x_v1; destruct (x =? v2)%N eqn:E_x_v2; try reflexivity.
+    rewrite N.eqb_eq in E_x_v1. rewrite E_x_v1 in E_x_v2. rewrite H_v1_neq_v2 in E_x_v2. discriminate.
+  Qed.
+
+  Lemma f_v1_v2_neq_fun:
+    forall (g : N -> EVMWord) (v1 v2:N) (w1 w2 : EVMWord),
+      (v1 =? v2)%N = false ->
+      (fun key : N => if (key =? v1)%N then w1 else if (key =? v2)%N then w2 else g key) 
+      =
+        (fun key : N => if (key =? v2)%N then w2 else if (key =? v1)%N then w1 else g key).
+  Proof.
+    intros g v1 v2 w1 w2 H_v1_neq_v2.
+    apply functional_extensionality.
+    apply f_v1_v2_neq.
+    apply H_v1_neq_v2.
+  Qed.
+
+  
+  Lemma swap_storage_update_snd:
+    forall ctx sstrg u1 u2 maxidx sb ops,
+      is_sat ctx ->
+      valid_sstorage maxidx sstrg ->
+      valid_sstorage_update maxidx u1 ->
+      valid_sstorage_update maxidx u2 ->
+      valid_bindings maxidx sb ops ->
+      swap_storage_update ctx u1 u2 maxidx sb = true ->
+      forall model mem strg exts, 
+             is_model ctx model = true ->
+             exists strg' : storage,
+               eval_sstorage (u1::u2::sstrg) maxidx sb model mem strg exts ops = Some strg' /\
+                 eval_sstorage (u2::u1::sstrg) maxidx sb model mem strg exts ops = Some strg'.
+  Proof.
+    intros ctx sstrg u1 u2 maxidx sb ops.
+    intros H_is_sat H_valid_sstrg H_valid_u1 H_valid_u2 H_valid_bs H_swap.
+    intros model mem strg exts H_is_model.
+    destruct u1 as [skey1 svalue1] eqn:E_u1.
+    destruct u2 as [skey2 svalue2] eqn:E_u2.
+    unfold swap_storage_update in H_swap.
+    destruct (follow_in_smap skey1 maxidx sb) eqn:E_follow_skey1; try discriminate; destruct f; destruct smv; try discriminate; destruct val eqn:E_v1; try discriminate.
+    
+    destruct (follow_in_smap skey2 maxidx sb) eqn:E_follow_skey2; try discriminate; destruct f; destruct smv; try discriminate; destruct val1 eqn:E_v2; try discriminate.
+ 
+    assert(H_swap' := H_swap).
+    rewrite N.ltb_lt in H_swap'.
+    pose proof (N.lt_neq (wordToN val2) (wordToN val0) H_swap') as H_swap_neq.
+    apply N.neq_sym in H_swap_neq.
+    rewrite <- N.eqb_neq in H_swap_neq.
+    
+    
+    assert(H_valid_u1' := H_valid_u1).
+    simpl in H_valid_u1'.
+    destruct H_valid_u1' as [H_valid_skey1 H_valid_svalue1].
+
+    assert(H_valid_u2' := H_valid_u2).
+    simpl in H_valid_u2'.
+    destruct H_valid_u2' as [H_valid_skey2 H_valid_svalue2].
+
+    
+    pose proof (eval_sstack_val'_succ (S maxidx) skey1 model mem strg exts maxidx sb ops H_valid_skey1 H_valid_bs (gt_Sn_n maxidx)) as H_eval_skey1.
+    destruct H_eval_skey1 as [skey1_v H_eval_skey1].
+
+    pose proof (eval_sstack_val'_succ (S maxidx) svalue1 model mem strg exts maxidx sb ops H_valid_svalue1 H_valid_bs (gt_Sn_n maxidx)) as H_eval_svalue1.
+    destruct H_eval_svalue1 as [svalue1_v H_eval_svalue1].
+
+    pose proof (eval_sstack_val'_succ (S maxidx) skey2 model mem strg exts maxidx sb ops H_valid_skey2 H_valid_bs (gt_Sn_n maxidx)) as H_eval_skey2.
+    destruct H_eval_skey2 as [skey2_v H_eval_skey2].
+
+    pose proof (eval_sstack_val'_succ (S maxidx) svalue2 model mem strg exts maxidx sb ops H_valid_svalue2 H_valid_bs (gt_Sn_n maxidx)) as H_eval_svalue2.
+    destruct H_eval_svalue2 as [svalue2_v H_eval_svalue2].
+ 
+    unfold eval_sstorage.
+    unfold map_option at 1.
+    rewrite <- map_option_ho.
+
+    unfold instantiate_storage_update at 1.
+    unfold eval_sstack_val at 1.
+    rewrite H_eval_skey1.
+    unfold eval_sstack_val at 1.
+    rewrite H_eval_svalue1.
+    
+    unfold instantiate_storage_update at 1.
+    unfold eval_sstack_val at 1.
+    rewrite H_eval_skey2.
+    unfold eval_sstack_val at 1.
+    rewrite H_eval_svalue2.
+
+    unfold eval_sstorage.
+    unfold map_option at 2.
+    rewrite <- map_option_ho.
+
+    unfold instantiate_storage_update at 2.
+    unfold eval_sstack_val at 2.
+    rewrite H_eval_skey2.
+    unfold eval_sstack_val at 2.
+    rewrite H_eval_svalue2.
+
+    unfold instantiate_storage_update at 2.
+    unfold eval_sstack_val at 2.
+    rewrite H_eval_skey1.
+    unfold eval_sstack_val at 2.
+    rewrite H_eval_svalue1.
+  
+    pose proof (eval_sstorage_succ maxidx sb model mem strg exts ops sstrg H_valid_sstrg H_valid_bs) as H_eval_sstrg.
+    destruct H_eval_sstrg as [strg' H_eval_sstrg].
+    unfold eval_sstorage in H_eval_sstrg.
+
+    destruct (map_option (instantiate_storage_update (fun sv : sstack_val => eval_sstack_val sv model mem strg exts maxidx sb ops)) sstrg) as [updates|] eqn:E_mo_eval_sstrg; try discriminate.
+
+    exists (fun key => if (key =? wordToN skey1_v)%N then svalue1_v else if (key =? wordToN skey2_v)%N then svalue2_v else strg' key).
+
+    simpl.
+
+    injection H_eval_sstrg as H_eval_sstrg.
+    rewrite H_eval_sstrg.
+ 
+    unfold concrete_interpreter.ConcreteInterpreter.sstore.
+    split; try reflexivity.
+   
+    unfold eval_sstack_val' in H_eval_skey1.
+    fold eval_sstack_val' in H_eval_skey1.
+    rewrite E_follow_skey1 in H_eval_skey1.
+    injection H_eval_skey1 as H_eval_skey1.
+
+    unfold eval_sstack_val' in H_eval_skey2.
+    fold eval_sstack_val' in H_eval_skey2.
+    rewrite E_follow_skey2 in H_eval_skey2.
+    injection H_eval_skey2 as H_eval_skey2.
+
+    rewrite H_eval_skey1 in H_swap_neq.
+    rewrite H_eval_skey2 in H_swap_neq.
+
+    pose proof (f_v1_v2_neq_fun strg' (wordToN skey1_v) (wordToN skey2_v) svalue1_v svalue2_v H_swap_neq) as H_f_v1_v2_neq_fun.
+
+    rewrite H_f_v1_v2_neq_fun.
+    reflexivity.
+Qed.
+
+  Lemma reorder_updates'_valid:
+    forall ctx maxidx sb ops,
+      valid_bindings maxidx sb ops ->
+      forall d sstrg b sstrg_r,
+      valid_sstorage maxidx sstrg ->
+      reorder_updates' d ctx sstrg maxidx sb = (b,sstrg_r) ->
+      valid_sstorage maxidx sstrg_r.
+  Proof.
+    intros ctx maxidx sb ops H_valid_sb.
+    induction d as [|d'' IHd'].
+    + intros sstrg b sstrg_r H_valid_sstrg H_reorder'.
+      simpl in H_reorder'.
+      injection H_reorder' as H_b H_sstrg_r.
+      rewrite <- H_sstrg_r.
+      apply H_valid_sstrg.
+    + intros sstrg b sstrg_r H_valid_sstrg H_reorder'.
+      simpl in H_reorder'.
+      destruct sstrg as [|u1 sstrg'] eqn:H_sstrg.
+      ++ injection H_reorder' as H_b H_sstrg_r.
+         rewrite <- H_sstrg_r.
+         simpl.
+         auto.
+      ++  destruct sstrg' as [|u2 sstrg''] eqn:H_sstrg'.
+          +++ injection H_reorder' as H_b H_sstrg_r.
+              rewrite <- H_sstrg_r.
+              simpl.
+              split; try auto.
+              apply H_valid_sstrg.
+          +++ destruct (swap_storage_update ctx u1 u2 maxidx sb) eqn:E_swap.
+              ++++ destruct (reorder_updates' d'' ctx (u1 :: sstrg'')) eqn:E_reorder'_rec.
+                   injection H_reorder' as H_b H_sstrg_r.
+                   rewrite <- H_sstrg_r.
+                   simpl in H_valid_sstrg.
+                   destruct H_valid_sstrg as [H_valid_u1 [H_valid_u2 H_valid_sstrg'']].
+                   pose proof (IHd' (u1 :: sstrg'') b0 s (valid_sstorage_when_extended_with_valid_update maxidx u1 sstrg'' H_valid_u1 H_valid_sstrg'') E_reorder'_rec) as IHd'_0.
+                   simpl.
+                   split.
+                   +++++ apply H_valid_u2.
+                   +++++ apply IHd'_0.
+              ++++ destruct (reorder_updates' d'' ctx (u2 :: sstrg'')) eqn:E_reorder'_rec.
+                   injection H_reorder' as H_b H_sstrg_r.
+                   rewrite <- H_sstrg_r.
+                   simpl in H_valid_sstrg.
+                   destruct H_valid_sstrg as [H_valid_u1 [H_valid_u2 H_valid_sstrg'']].
+                   pose proof (IHd' (u2 :: sstrg'') b0 s (valid_sstorage_when_extended_with_valid_update maxidx u2 sstrg'' H_valid_u2 H_valid_sstrg'') E_reorder'_rec) as IHd'_0.
+                   simpl.
+                   split.
+                   +++++ apply H_valid_u1.
+                   +++++ apply IHd'_0.
+  Qed.
+ 
+  Lemma reorder_updates'_snd:
+    forall ctx maxidx sb ops,
+      is_sat ctx ->
+      valid_bindings maxidx sb ops ->
+      forall d sstrg b sstrg_r,
+      valid_sstorage maxidx sstrg ->
+      reorder_updates' d ctx sstrg maxidx sb = (b,sstrg_r) ->
+      forall model mem strg exts, 
+             is_model ctx model = true ->
+             exists strg' : storage,
+               eval_sstorage sstrg maxidx sb model mem strg exts ops = Some strg' /\
+                 eval_sstorage sstrg_r maxidx sb model mem strg exts ops = Some strg'.
+  Proof.
+    intros ctx maxidx sb ops H_is_sat H_valid_sb.
+    induction d as [|d' IHd'].
+    + intros sstrg b sstrg_r H_valid_sstrg H_reorder'.
+      intros model mem strg exts H_is_model.
+      simpl in H_reorder'.
+      injection H_reorder' as H_b H_sstrg_r.
+      rewrite <- H_sstrg_r.
+      pose proof (eval_sstorage_succ maxidx sb model mem strg exts ops sstrg H_valid_sstrg H_valid_sb) as H_eval_sstrg.
+      destruct H_eval_sstrg as [strg' H_eval_sstrg].
+      exists strg'.
+      split; apply H_eval_sstrg.
+    + intros sstrg b sstrg_r H_valid_sstrg H_reorder'.
+      intros model mem strg exts H_is_model.
+      simpl in H_reorder'.
+      destruct sstrg as [|u1 sstrg'] eqn:E_sstrg.
+      ++ injection H_reorder' as H_b H_sstrg_r.
+         rewrite <- H_sstrg_r.
+         exists strg.
+         unfold eval_sstorage.
+         simpl.
+         split; reflexivity.
+      ++ destruct sstrg' as [|u2 sstrg''] eqn:E_sstrg'.
+         +++ injection H_reorder' as H_b H_sstrg_r.
+             rewrite <- H_sstrg_r.
+             destruct u1 as [skey1 svalue1] eqn:E_u1.
+             simpl in H_valid_sstrg.
+             destruct H_valid_sstrg as [[H_valid_skey1 H_valid_svalue1] _].
+
+             pose proof (eval_sstack_val'_succ (S maxidx) skey1 model mem strg exts maxidx sb ops H_valid_skey1 H_valid_sb (gt_Sn_n maxidx)) as E_eval_skey1.
+             destruct E_eval_skey1 as [skey1_v E_eval_skey1].
+             pose proof (eval_sstack_val'_succ (S maxidx) svalue1 model mem strg exts maxidx sb ops H_valid_svalue1 H_valid_sb (gt_Sn_n maxidx)) as E_eval_svalue1.
+             destruct E_eval_svalue1 as [svalue1_v E_eval_svalue1].
+
+             exists (fun key => if (key =? wordToN skey1_v)%N then svalue1_v else strg key).
+             unfold eval_sstorage.
+             unfold map_option.
+             unfold instantiate_storage_update.
+             unfold eval_sstack_val.
+             rewrite E_eval_skey1.
+             rewrite E_eval_svalue1.
+             unfold update_storage.
+             split; reflexivity.
+         +++ destruct (swap_storage_update ctx u1 u2 maxidx sb) eqn:E_swap.
+             ++++ destruct (reorder_updates' d' ctx (u1 :: sstrg'') maxidx sb) as [b' sstrg_r'] eqn:E_reorder'_rec.
+                  injection H_reorder' as E_b E_sstrg_r.
+
+                  simpl in H_valid_sstrg.
+                  destruct H_valid_sstrg as [H_valid_u1 [H_valid_u2 H_valid_sstrg'']].
+                   
+                  pose proof (swap_storage_update_snd  ctx sstrg'' u1 u2 maxidx sb ops H_is_sat H_valid_sstrg'' H_valid_u1 H_valid_u2 H_valid_sb E_swap model mem strg exts H_is_model) as H_swap_storage_update_snd.
+
+                  destruct H_swap_storage_update_snd as [strg_aux [H_eval_u1_u2_sstrg'' H_eval_u2_u1_sstrg'' ]].
+		  rewrite <- H_eval_u2_u1_sstrg'' in H_eval_u1_u2_sstrg''.
+                  rewrite H_eval_u1_u2_sstrg''.
+ 
+                  pose proof (IHd' (u1 :: sstrg'') b' sstrg_r' (valid_sstorage_when_extended_with_valid_update maxidx u1 sstrg'' H_valid_u1 H_valid_sstrg'') E_reorder'_rec model mem strg exts H_is_model) as IHd'_0.
+                  destruct IHd'_0 as [strg' [H_eval_u1_sstrg'' H_eval_sstrg_r']].
+                  rewrite <- E_sstrg_r.
+                  
+                  unfold eval_sstorage in H_eval_u1_sstrg''.
+                  destruct (map_option (instantiate_storage_update (fun sv : sstack_val => eval_sstack_val sv model mem strg exts maxidx sb ops)) (u1 :: sstrg'')) as [updates1|] eqn:E_mo_1; try discriminate.
+                  
+                  unfold eval_sstorage in H_eval_sstrg_r'.
+                  destruct (map_option (instantiate_storage_update (fun sv : sstack_val => eval_sstack_val sv model mem strg exts maxidx sb ops)) sstrg_r') as [updates2|] eqn:E_mo_2; try discriminate.
+                  
+                  destruct u2 as [skey2 svalue2] eqn:E_u2.
+                  simpl in H_valid_u2.
+                  destruct H_valid_u2 as [H_valid_skey2 H_valid_svalue2].
+
+                  pose proof (eval_sstack_val'_succ (S maxidx) skey2 model mem strg exts maxidx sb ops H_valid_skey2 H_valid_sb (gt_Sn_n maxidx)) as E_eval_skey2.
+                  destruct E_eval_skey2 as [skey2_v E_eval_skey2].
+                  pose proof (eval_sstack_val'_succ (S maxidx) svalue2 model mem strg exts maxidx sb ops H_valid_svalue2 H_valid_sb (gt_Sn_n maxidx)) as E_eval_svalue2.
+                  destruct E_eval_svalue2 as [svalue2_v E_eval_svalue2].
+                  
+                  unfold eval_sstorage.
+                  unfold map_option.
+                  repeat rewrite <- map_option_ho.
+                  
+                  unfold instantiate_storage_update at 1.
+                  unfold eval_sstack_val at 1.
+                  rewrite E_eval_skey2.
+                  unfold eval_sstack_val at 1.
+                  rewrite E_eval_svalue2.
+                  
+                  unfold instantiate_storage_update at 3.
+                  unfold eval_sstack_val at 3.
+                  rewrite E_eval_skey2.
+                  unfold eval_sstack_val at 3.
+                  rewrite E_eval_svalue2.
+
+                  unfold map_option in E_mo_1.
+                  destruct (instantiate_storage_update (fun sv : sstack_val => eval_sstack_val sv model mem strg exts maxidx sb ops) u1) as [elem_val|] eqn:E_elem_val; try discriminate.
+                  
+                  repeat rewrite <- map_option_ho in E_mo_1.
+                  rewrite E_mo_1.
+                  rewrite E_mo_2.
+
+                  unfold update_storage.
+                  fold update_storage.
+
+                  injection H_eval_u1_sstrg'' as H_eval_u1_sstrg''.
+                  rewrite H_eval_u1_sstrg''.
+                  injection H_eval_sstrg_r' as H_eval_sstrg_r'.
+                  rewrite H_eval_sstrg_r'.
+
+                  exists (update_storage' strg' (U_SSTORE EVMWord skey2_v svalue2_v)).
+                  split; reflexivity.
+                  
+             ++++ destruct (reorder_updates' d' ctx (u2 :: sstrg'') maxidx sb) as [b' sstrg_r'] eqn:E_reorder'_rec.
+                  simpl in H_valid_sstrg.
+                  destruct H_valid_sstrg as [H_valid_u1 [H_valid_u2 H_valid_sstrg'']].
+
+                  pose proof (IHd' (u2 :: sstrg'') b' sstrg_r' (valid_sstorage_when_extended_with_valid_update maxidx u2 sstrg'' H_valid_u2 H_valid_sstrg'') E_reorder'_rec model mem strg exts H_is_model) as IHd'_0.
+                  destruct IHd'_0 as [strg' [H_eval_u2_sstrg'' H_eval_sstrg_r']].
+                  injection H_reorder' as H_b' H_sstrg_r'.
+                  rewrite <- H_sstrg_r'.
+
+                  unfold eval_sstorage in H_eval_u2_sstrg''.
+                  destruct (map_option (instantiate_storage_update (fun sv : sstack_val => eval_sstack_val sv model mem strg exts maxidx sb ops)) (u2 :: sstrg'')) as [updates1|] eqn:E_mo_1; try discriminate.
+                  
+                  unfold eval_sstorage in H_eval_sstrg_r'.
+                  destruct (map_option (instantiate_storage_update (fun sv : sstack_val => eval_sstack_val sv model mem strg exts maxidx sb ops)) sstrg_r') as [updates2|] eqn:E_mo_2; try discriminate.
+                  
+                  destruct u1 as [skey1 svalue1] eqn:E_u1.
+                  simpl in H_valid_u1.
+                  destruct H_valid_u1 as [H_valid_skey1 H_valid_svalue1].
+
+                  pose proof (eval_sstack_val'_succ (S maxidx) skey1 model mem strg exts maxidx sb ops H_valid_skey1 H_valid_sb (gt_Sn_n maxidx)) as E_eval_skey1.
+                  destruct E_eval_skey1 as [skey1_v E_eval_skey1].
+                  pose proof (eval_sstack_val'_succ (S maxidx) svalue1 model mem strg exts maxidx sb ops H_valid_svalue1 H_valid_sb (gt_Sn_n maxidx)) as E_eval_svalue1.
+                  destruct E_eval_svalue1 as [svalue1_v E_eval_svalue1].
+                  
+                  unfold eval_sstorage.
+                  unfold map_option.
+                  repeat rewrite <- map_option_ho.
+                  
+                  unfold instantiate_storage_update at 1.
+                  unfold eval_sstack_val at 1.
+                  rewrite E_eval_skey1.
+                  unfold eval_sstack_val at 1.
+                  rewrite E_eval_svalue1.
+                  
+                  unfold instantiate_storage_update at 3.
+                  unfold eval_sstack_val at 3.
+                  rewrite E_eval_skey1.
+                  unfold eval_sstack_val at 3.
+                  rewrite E_eval_svalue1.
+
+                  unfold map_option in E_mo_1.
+                  destruct (instantiate_storage_update (fun sv : sstack_val => eval_sstack_val sv model mem strg exts maxidx sb ops) u2) as [elem_val|] eqn:E_elem_val; try discriminate.
+                  
+                  repeat rewrite <- map_option_ho in E_mo_1.
+                  rewrite E_mo_1.
+                  rewrite E_mo_2.
+
+                  unfold update_storage.
+                  fold update_storage.
+
+                  injection H_eval_u2_sstrg'' as H_eval_u2_sstrg''.
+                  rewrite H_eval_u2_sstrg''.
+                  injection H_eval_sstrg_r' as H_eval_sstrg_r'.
+                  rewrite H_eval_sstrg_r'.
+
+                  exists (update_storage' strg' (U_SSTORE EVMWord skey1_v svalue1_v)).
+                  split; reflexivity.
+  Qed.
+
+
+  Lemma reorder_storage_updates_valid:
+    forall ctx maxidx sb ops,
+      valid_bindings maxidx sb ops ->
+      forall d n sstrg sstrg_r,
+      valid_sstorage maxidx sstrg ->
+      reorder_storage_updates d n ctx sstrg maxidx sb = sstrg_r ->
+      valid_sstorage  maxidx sstrg_r.
+  Proof.
+    intros ctx maxidx sb ops H_valid_sb.
+    induction d as [|d' IHd'].
+    + intros n sstrg sstrg' H_valid_sstrg H_reorder.
+      simpl in H_reorder.
+      rewrite <- H_reorder.
+      apply H_valid_sstrg.
+    + intros n sstrg sstrg_r H_valid_sstrg H_reorder.
+      unfold reorder_storage_updates in H_reorder.
+      fold reorder_storage_updates in H_reorder.
+      destruct (reorder_updates' n ctx sstrg maxidx sb) as [changed sstrg'] eqn:E_reorder_update'.
+      pose proof (reorder_updates'_valid ctx maxidx sb ops H_valid_sb n sstrg changed sstrg' H_valid_sstrg E_reorder_update') as H_valid_sstrg'.
+      destruct changed.
+      ++ pose proof (IHd' n sstrg' sstrg_r H_valid_sstrg' H_reorder) as H_valid_sstrg_r.
+         apply H_valid_sstrg_r.
+      ++ rewrite <- H_reorder.
+         apply H_valid_sstrg'.
+Qed.
+
+
+
+  Lemma reorder_storage_updates_snd:
+    forall ctx maxidx sb ops,
+      is_sat ctx ->
+      valid_bindings maxidx sb ops ->
+      forall d n sstrg sstrg_r,
+        valid_sstorage maxidx sstrg ->
+      reorder_storage_updates d n ctx sstrg maxidx sb = sstrg_r ->
+      forall model mem strg exts,
+        is_model ctx model = true ->
+        exists strg' : storage,
+          eval_sstorage sstrg maxidx sb model mem strg exts ops = Some strg' /\
+            eval_sstorage sstrg_r maxidx sb model mem strg exts ops = Some strg'.
+  Proof.
+    intros ctx maxidx sb ops H_is_sat H_valid_sb.
+    induction d as [|d' IHd'].
+    + intros n sstrg sstrg' H_valid_sstrg H_reorder stk mem strg exts H_is_model.
+      simpl in H_reorder.
+      rewrite <- H_reorder.
+      pose proof (eval_sstorage_succ maxidx sb stk mem strg exts ops sstrg H_valid_sstrg H_valid_sb) as H_eval_sstrg.
+      destruct H_eval_sstrg as [strg' H_eval_sstrg].
+      exists strg'.
+      split; apply H_eval_sstrg.
+    + intros n sstrg sstrg' H_valid_sstrg H_reorder stk mem strg exts H_is_model.
+      simpl in H_reorder.
+      destruct (reorder_updates' n ctx sstrg maxidx sb) as [changed sstrg_r] eqn:E_reorder_updates'.
+     
+      pose proof (reorder_updates'_snd ctx maxidx sb ops H_is_sat H_valid_sb n sstrg changed sstrg_r H_valid_sstrg E_reorder_updates' stk mem strg exts H_is_model) as H_reorder_updates'_snd.
+      destruct H_reorder_updates'_snd as [strg' [H_eval_sstrg H_eval_sstrg_r]].
+      
+      destruct changed eqn:E_changed.
+      ++ pose proof (reorder_updates'_valid ctx maxidx sb ops H_valid_sb n sstrg true sstrg_r H_valid_sstrg E_reorder_updates') as H_valid_sstrg_r.
+
+         pose proof (IHd' n sstrg_r sstrg' H_valid_sstrg_r H_reorder stk mem strg exts H_is_model) as IHd'_0.
+         destruct IHd'_0 as [strg'' [H_eval_sstrg_r_bis H_eval_sstrg']].
+         exists strg'.
+
+         rewrite H_eval_sstrg_r in H_eval_sstrg_r_bis.
+         injection H_eval_sstrg_r_bis as H_strg'_eq_strg''.
+         rewrite <- H_strg'_eq_strg'' in H_eval_sstrg'.
+         split.
+         +++ apply H_eval_sstrg.
+         +++ apply H_eval_sstrg'.
+         
+      ++ rewrite <- H_reorder.
+         exists strg'.
+         split.
+         +++ apply H_eval_sstrg.
+         +++ apply H_eval_sstrg_r.
+  Qed.
+
+  
+  Theorem po_storage_cmp_snd:
+    safe_sstorage_cmp_ext_wrt_sstack_value_cmp po_storage_cmp.
+  Proof.
+    unfold safe_sstorage_cmp_ext_wrt_sstack_value_cmp.
+    unfold safe_sstorage_cmp_ext_d.
+    unfold safe_sstorage_cmp.
+    intros d sstack_val_cmp H_sstack_val_cmp_snd d' H_d'_le_d ctx sstrg1 sstrg2 maxidx1 sb1 maxidx2 sb2 ops H_is_sat H_valid_sb1 H_valid_sb2 H_valid_sstrg1 H_valid_sstrg2 H_po_cmp stk mem strg exts H_is_model.
+    unfold po_storage_cmp in H_po_cmp.
+    destruct (length sstrg1 =? length sstrg2); try discriminate.
+
+    remember (reorder_storage_updates (length sstrg1) (length sstrg1) ctx sstrg1 maxidx1 sb1) as sstrg1_r.
+    remember (reorder_storage_updates (length sstrg2) (length sstrg2) ctx sstrg2 maxidx2 sb2) as sstrg2_r.
+    
+    pose proof (reorder_storage_updates_snd ctx maxidx1 sb1 ops H_is_sat H_valid_sb1 (length sstrg1) (length sstrg1) sstrg1 sstrg1_r H_valid_sstrg1 (eq_sym Heqsstrg1_r) stk mem strg exts H_is_model) as H_reorder_storage_updates_snd_sstrg1_r.
+    pose proof (reorder_storage_updates_valid ctx maxidx1 sb1 ops H_valid_sb1 (length sstrg1) (length sstrg1) sstrg1 sstrg1_r H_valid_sstrg1 (eq_sym Heqsstrg1_r)) as H_valid_sstrg1_r.
+
+    destruct H_reorder_storage_updates_snd_sstrg1_r as [strg1' [H_eval_sstrg1 H_eval_sstrg1_r]].
+
+    pose proof (reorder_storage_updates_snd ctx maxidx2 sb2 ops H_is_sat H_valid_sb2 (length sstrg2) (length sstrg2) sstrg2 sstrg2_r H_valid_sstrg2 (eq_sym Heqsstrg2_r) stk mem strg exts H_is_model) as H_reorder_storage_updates_snd_sstrg2_r.
+    pose proof (reorder_storage_updates_valid ctx maxidx2 sb2 ops H_valid_sb2 (length sstrg2) (length sstrg2) sstrg2 sstrg2_r H_valid_sstrg2 (eq_sym Heqsstrg2_r)) as H_valid_sstrg2_r.
+
+    destruct H_reorder_storage_updates_snd_sstrg2_r as [strg2' [H_eval_sstrg2 H_eval_sstrg2_r]].
+
+    pose proof (basic_storage_cmp_snd) as H_basic_storage_cmp_snd.
+    unfold safe_sstorage_cmp_ext_wrt_sstack_value_cmp in H_basic_storage_cmp_snd.
+    unfold safe_sstorage_cmp_ext_d in H_basic_storage_cmp_snd.
+    unfold safe_sstorage_cmp in H_basic_storage_cmp_snd.
+
+    pose proof (H_basic_storage_cmp_snd d sstack_val_cmp H_sstack_val_cmp_snd d' H_d'_le_d ctx sstrg1_r sstrg2_r maxidx1 sb1 maxidx2 sb2 ops H_is_sat H_valid_sb1 H_valid_sb2 H_valid_sstrg1_r H_valid_sstrg2_r H_po_cmp stk mem strg exts H_is_model) as H_basic_cmp_snd.
+
+    destruct H_basic_cmp_snd as [strg' [H_eval_sstrg1_r_bis H_eval_sstrg2_r_bis]].
+    exists strg1'.
+    split.
+    + apply H_eval_sstrg1.
+    + rewrite H_eval_sstrg2.
+      rewrite H_eval_sstrg2_r_bis in H_eval_sstrg2_r.
+      injection H_eval_sstrg2_r as H_eval_sstrg2_r.
+      rewrite H_eval_sstrg1_r_bis in H_eval_sstrg1_r.
+      injection H_eval_sstrg1_r as H_eval_sstrg1_r.
+      rewrite <- H_eval_sstrg2_r.
+      rewrite <- H_eval_sstrg1_r.
+      reflexivity.
+  Qed.
+
+    
+
+
+End StorageCmpImplSoundness.
